ulib/FStar.Pointer.fst
@@ -7,84 +7,321 @@ module HST = FStar.ST
 
 type array (length: UInt32.t) (t: Type) = (s: Seq.seq t {Seq.length s == UInt32.v length})
 
-noeq private type step: (from: Type) -> (to: Type) -> Tot Type =
+type base_typ =
+| TUInt8
+| TUInt16
+| TUInt32
+| TUInt64
+| TInt8
+| TInt16
+| TInt32
+| TInt64
+| TChar
+| TBool
+
+type typ =
+| TBase:
+  (b: base_typ) ->
+  typ
+| TStruct:
+  (l: struct_typ) ->
+  typ
+| TArray:
+  (length: UInt32.t) ->
+  (t: typ) ->
+  typ
+| TPointer:
+  (t: typ) ->
+  typ
+and struct_typ = (l: list (string * typ) { List.Tot.noRepeats (List.Tot.map fst l) })
+
+let rec typ_depth
+  (t: typ)
+: Tot nat
+= match t with
+  | TArray _ t -> 1 + typ_depth t
+  | TStruct l -> 1 + struct_typ_depth l
+  | _ -> 0
+and struct_typ_depth
+  (l: struct_typ)
+: Tot nat
+= match l with
+  | [] -> 0
+  | (_, t) :: l ->
+    let n1 = typ_depth t in
+    let n2 = struct_typ_depth l in
+    if n1 > n2 then n1 else n2
+
+let struct_field
+  (l: struct_typ)
+: Tot eqtype
+= (s: string { List.Tot.mem s (List.Tot.map fst l) } )
+
+let typ_of_struct_field
+  (l: struct_typ)
+  (f: struct_field l)
+: Tot (t: typ {t << l})
+= List.Tot.assoc_mem f l;
+  let y = Some?.v (List.Tot.assoc f l) in
+  List.Tot.assoc_precedes f l y;
+  y
+
+let rec typ_depth_typ_of_struct_field
+  (l: struct_typ)
+  (f: struct_field l)
+: Lemma
+  (ensures (typ_depth (typ_of_struct_field l f) <= struct_typ_depth l))
+  (decreases l)
+= let ((f', _) :: l') = l in
+  if f = f'
+  then ()
+  else begin
+    let f: string = f in
+    assert (List.Tot.mem f (List.Tot.map fst l'));
+    List.Tot.assoc_mem f l';
+    typ_depth_typ_of_struct_field l' f
+  end
+
+private type step: (from: typ) -> (to: typ) -> Tot Type0 =
   | StepField:
-    (key: eqtype) ->
-    (value: ((k: key) -> Tot Type)) ->
-    (fd: key) ->
-    step (DM.t key value) (value fd)
+    (l: struct_typ) ->
+    (fd: struct_field l) ->
+    step (TStruct l) (typ_of_struct_field l fd)
   | StepCell:
     (length: UInt32.t) ->
-    (value: Type) ->
+    (value: typ) ->
     (index: UInt32.t { UInt32.v index < UInt32.v length } ) ->
-    step (array length value) value
+    step (TArray length value) value
 
-noeq private type path (from: Type) : (to: Type) -> Tot Type =
+private type path (from: typ) : (to: typ) -> Tot Type0 =
   | PathBase:
     path from from
   | PathStep:
-    (through: Type) ->
-    (to: Type) ->
+    (through: typ) ->
+    (to: typ) ->
     (p: path from through) ->
     (s: step through to) ->
     path from to
 
-private let rec path_sel
-  (#from: Type)
-  (#to: Type)
-  (m: from)
+private let step_typ_depth
+  (#from #to: typ)
+  (s: step from to)
+: Lemma
+  (typ_depth from > typ_depth to)
+= match s with
+  | StepField l fd ->
+    typ_depth_typ_of_struct_field l fd
+  | _ -> ()
+
+private let rec path_typ_depth
+  (#from #to: typ)
   (p: path from to)
-: Tot to
+: Lemma
+  (ensures (
+    typ_depth from >= typ_depth to /\ (
+      (~ (PathBase? p)) ==> typ_depth from <> typ_depth to
+  )))
+  (decreases p)
+= match p with
+  | PathBase -> ()
+  | PathStep _ _ p' s ->
+    path_typ_depth p';
+    step_typ_depth s
+
+(*
+private
+let not_cell
+  (#from #to: typ)
+  (p: path from to)
+: GTot bool
+= match p with
+  | PathStep _ _ _ (StepCell _ _ _) -> false
+  | _ -> true
+
+private type array_path (from: typ) (to_elem: typ) : (length: UInt32.t) -> Tot Type0 =
+| PSingleton:
+  (p: path from to_elem { not_cell p } ) ->
+  array_path from to_elem 1ul
+| PArray:
+  length: UInt32.t ->
+  path from (TArray length to_elem) ->
+  array_path from to_elem length
+
+private let path' (from: typ) (to: typ) : Tot Type0 =
+  if TArray? to
+  then
+    let length = TArray?.length to in
+    (array_path from (TArray?.t to) length * (offset: UInt32.t & (length': UInt32.t {UInt32.v offset + UInt32.v length' <= UInt32.v length})))
+  else path from to
+*)
+
+let type_of_base_typ
+  (t: base_typ)
+: Tot Type0
+= match t with
+  | TUInt8 -> FStar.UInt8.t
+  | TUInt16 -> FStar.UInt16.t
+  | TUInt32 -> FStar.UInt32.t
+  | TUInt64 -> FStar.UInt64.t
+  | TInt8 -> FStar.Int8.t
+  | TInt16 -> FStar.Int16.t
+  | TInt32 -> FStar.Int32.t
+  | TInt64 -> FStar.Int64.t
+  | TChar -> FStar.Char.char
+  | TBool -> bool
+
+(** Pointers to data of type t *)
+
+noeq private type _pointer (to : typ): Type0 =
+  | Pointer:
+    (from: typ) ->
+    (contents: HS.aref) ->
+    (p: path from to) ->
+    _pointer to
+
+abstract let pointer (t: typ): Tot Type0 =
+  _pointer t
+
+let type_of_struct_field'
+  (l: struct_typ)
+  (type_of_typ: (
+    (t: typ { t << l } ) ->
+    Tot Type0
+  ))
+  (f: struct_field l)
+: Tot Type0 =
+  List.Tot.assoc_mem f l;
+  let y = typ_of_struct_field l f in
+  List.Tot.assoc_precedes f l y;
+  type_of_typ y
+
+let rec type_of_typ
+  (t: typ)
+: Tot Type0
+= match t with
+  | TBase b -> type_of_base_typ b
+  | TStruct l ->
+    DM.t (struct_field l) (type_of_struct_field' l type_of_typ)
+  | TArray length t ->
+    array length (type_of_typ t)
+  | TPointer t ->
+    pointer t
+
+let type_of_struct_field
+  (l: struct_typ)
+: Tot (struct_field l -> Tot Type0)
+= type_of_struct_field' l type_of_typ
+
+let struct (l: struct_typ) = DM.t (struct_field l) (type_of_struct_field l)
+
+let type_of_typ_struct
+  (l: struct_typ)
+: Lemma
+  (type_of_typ (TStruct l) == struct l)
+  [SMTPat (type_of_typ (TStruct l))]
+= assert_norm (type_of_typ (TStruct l) == struct l)
+
+let typ_of_type_type_of_struct_field
+  (l: struct_typ)
+  (f: struct_field l)
+: Lemma
+  (type_of_typ (typ_of_struct_field l f) == type_of_struct_field l f)
+  [SMTPat (type_of_typ (typ_of_struct_field l f))]
+= ()
+
+let struct_sel (#l: struct_typ) (s: struct l) (f: struct_field l) : Tot (type_of_struct_field l f) =
+  DM.sel s f
+
+let struct_upd (#l: struct_typ) (s: struct l) (f: struct_field l) (v: type_of_struct_field l f) : Tot (struct l) =
+  DM.upd s f v
+
+let struct_create (#l: struct_typ) (f: ((fd: struct_field l) -> Tot (type_of_struct_field l fd))) : Tot (struct l) =
+  DM.create #(struct_field l) #(type_of_struct_field l) f
+
+private
+let rec dummy_val
+  (t: typ)
+: Tot (type_of_typ t)
+= match t with
+  | TBase b ->
+    begin match b with
+    | TUInt8 -> UInt8.uint_to_t 0
+    | TUInt16 -> UInt16.uint_to_t 0
+    | TUInt32 -> UInt32.uint_to_t 0
+    | TUInt64 -> UInt64.uint_to_t 0
+    | TInt8 -> Int8.int_to_t 0
+    | TInt16 -> Int16.int_to_t 0
+    | TInt32 -> Int32.int_to_t 0
+    | TInt64 -> Int64.int_to_t 0
+    | TChar -> 'c'
+    | TBool -> false
+    end
+  | TStruct l ->
+    struct_create (fun f -> (
+      dummy_val (typ_of_struct_field l f)
+    ))
+  | TArray length t -> Seq.create (UInt32.v length) (dummy_val t)
+  | TPointer t -> Pointer t HS.dummy_aref PathBase
+
+private let rec path_sel
+  (#from: typ)
+  (#to: typ)
+  (m: type_of_typ from)
+  (p: path from to)
+: Tot (type_of_typ to)
+  (decreases p)
 = match p with
   | PathBase -> m
   | PathStep through' to' p' s ->
-    let (m': through') = path_sel m p' in
+    let (m': type_of_typ through') = path_sel m p' in
     begin match s with
-    | StepField key value fd ->
-      let (m': DM.t key value) = m' in
-      DM.sel m' fd
+    | StepField l fd ->
+      let (m': struct l) = m' in
+      struct_sel m' fd
     | StepCell length value i -> Seq.index m' (UInt32.v i)
     end
 
 private let rec path_upd
-  (#from: Type)
-  (#to: Type)
-  (m: from)
+  (#from: typ)
+  (#to: typ)
+  (m: type_of_typ from)
   (p: path from to)
-  (v: to)
-: Tot from
+  (v: type_of_typ to)
+: Tot (type_of_typ from)
+  (decreases p)
 = match p with
   | PathBase -> v
   | PathStep through' to' p' st ->
-    let (s: through') = path_sel m p' in
-    let (s': through') = match st with
-    | StepField key value fd ->
-      let (s: DM.t key value) = s in
-      DM.upd s fd v
+    let (s: type_of_typ through') = path_sel m p' in
+    let (s': type_of_typ through') = match st with
+    | StepField l fd ->
+      let (s: struct l) = s in
+      struct_upd s fd v
     | StepCell length value i ->
       Seq.upd s (UInt32.v i) v
     in
     path_upd m p' s'
 
 private let rec path_sel_upd_same
-  (#from: Type)
-  (#to: Type)
-  (m: from)
+  (#from: typ)
+  (#to: typ)
+  (m: type_of_typ from)
   (p: path from to)
-  (v: to)
+  (v: type_of_typ to)
 : Lemma
   (requires True)
   (ensures (path_sel (path_upd m p v) p == v))
+  (decreases p)
   [SMTPat (path_sel (path_upd m p v) p)]
 = match p with
   | PathBase -> ()
   | PathStep through' to' p' st ->
-    let (s: through') = path_sel m p' in
-    let (s': through') = match st with
-    | StepField key value fd ->
-      let (s: DM.t key value) = s in
+    let (s: type_of_typ through') = path_sel m p' in
+    let (s': type_of_typ through') = match st with
+    | StepField l fd ->
+      let (s: struct l) = s in
       let _ = DM.sel_upd_same s fd v in
-      DM.upd s fd v
+      struct_upd s fd v
     | StepCell length value i ->
       let s' = Seq.upd s (UInt32.v i) v in
       Seq.lemma_index_upd1 s (UInt32.v i) v;
@@ -93,9 +330,9 @@ private let rec path_sel_upd_same
     path_sel_upd_same m p' s'
 
 private let rec path_concat
-  (#from: Type)
-  (#through: Type)
-  (#to: Type)
+  (#from: typ)
+  (#through: typ)
+  (#to: typ)
   (p: path from through)
   (q: path through to)
 : Pure (path from to)
@@ -107,27 +344,28 @@ private let rec path_concat
   | PathStep through' to' q' st -> PathStep through' to' (path_concat p q') st
 
 private let path_concat_base_r
-  (#from: Type)
-  (#to: Type)
+  (#from: typ)
+  (#to: typ)
   (p: path from to)
 : Lemma
   (ensures (path_concat p PathBase == p))
 = ()
 
 private let rec path_concat_base_l
-  (#from: Type)
-  (#to: Type)
+  (#from: typ)
+  (#to: typ)
   (p: path from to)
 : Lemma
   (requires True)
   (ensures (path_concat PathBase p == p))
+  (decreases p)
   [SMTPat (path_concat PathBase p)]
 = match p with
   | PathBase -> ()
   | PathStep _ _ p' _ -> path_concat_base_l p'
 
 private let rec path_concat_assoc
-  (#t0 #t1 #t2 #t3: Type)
+  (#t0 #t1 #t2 #t3: typ)
   (p01: path t0 t1)
   (p12: path t1 t2)
   (p23: path t2 t3)
@@ -140,10 +378,10 @@ private let rec path_concat_assoc
   | PathStep _ _ p23' _ -> path_concat_assoc p01 p12 p23'
 
 private let rec path_sel_concat
-  (#from: Type)
-  (#through: Type)
-  (#to: Type)
-  (m: from)
+  (#from: typ)
+  (#through: typ)
+  (#to: typ)
+  (m: type_of_typ from)
   (p: path from through)
   (q: path through to)
 : Lemma
@@ -156,13 +394,13 @@ private let rec path_sel_concat
   | PathStep _ _ q' _ -> path_sel_concat m p q'
 
 private let rec path_upd_concat
-  (#from: Type)
-  (#through: Type)
-  (#to: Type)
-  (m: from)
+  (#from: typ)
+  (#through: typ)
+  (#to: typ)
+  (m: type_of_typ from)
   (p: path from through)
   (q: path through to)
-  (v: to)
+  (v: type_of_typ to)
 : Lemma
   (requires True)
   (ensures (path_upd m (path_concat p q) v == path_upd m p (path_upd (path_sel m p) q v)))
@@ -171,11 +409,11 @@ private let rec path_upd_concat
 = match q with
   | PathBase -> ()
   | PathStep through' to' q' st ->
-    let (s: through') = path_sel m (path_concat p q') in
-    let (s': through') = match st with
-    | StepField key value fd ->
-      let (s:DM.t key value) = s in
-      DM.upd s fd v
+    let (s: type_of_typ through') = path_sel m (path_concat p q') in
+    let (s': type_of_typ through') = match st with
+    | StepField l fd ->
+      let (s: struct l) = s in
+      struct_upd s fd v
     | StepCell length value i ->
       Seq.upd s (UInt32.v i) v
     in
@@ -183,34 +421,35 @@ private let rec path_upd_concat
 
 // TODO: rename as: prefix_of; use infix notation (p1 `prefix_of` p2)
 private let rec path_includes
-  (#from: Type)
-  (#to1 #to2: Type)
+  (#from: typ)
+  (#to1 #to2: typ)
   (p1: path from to1)
   (p2: path from to2)
-: Ghost Type0
+: Ghost bool
   (requires True)
   (ensures (fun _ -> True))
   (decreases p2)
-= (to1 == to2 /\ p1 == p2) \/ (match p2 with
-  | PathBase -> False
+= (to1 = to2 && p1 = p2) || (match p2 with
+  | PathBase -> false
   | PathStep _ _ p2' _ ->
     path_includes p1 p2'
   )
 
 private let rec path_includes_base
-  (#from: Type)
-  (#to: Type)
+  (#from: typ)
+  (#to: typ)
   (p: path from to)
 : Lemma
   (requires True)
   (ensures (path_includes (PathBase #from) p))
+  (decreases p)
   [SMTPat (path_includes PathBase p)]
 = match p with
   | PathBase -> ()
   | PathStep _ _ p2' _ -> path_includes_base p2'
 
 private let path_includes_refl
-  (#from #to: Type)
+  (#from #to: typ)
   (p: path from to)
 : Lemma
   (requires True)
@@ -219,7 +458,7 @@ private let path_includes_refl
 = ()
 
 private let path_includes_step_r
-  (#from #through #to: Type)
+  (#from #through #to: typ)
   (p: path from through)
   (s: step through to)
 : Lemma
@@ -229,7 +468,7 @@ private let path_includes_step_r
 = ()
 
 private let rec path_includes_trans
-  (#from #to1 #to2 #to3: Type)
+  (#from #to1 #to2 #to3: typ)
   (p1: path from to1)
   (p2: path from to2)
   (p3: path from to3  {path_includes p1 p2 /\ path_includes p2 p3})
@@ -252,32 +491,32 @@ private let rec path_includes_trans
     )
 
 private let rec path_includes_ind
-  (#from: Type)
-  (x: (#to1: Type) ->
-      (#to2: Type) ->
+  (#from: typ)
+  (x: (#to1: typ) ->
+      (#to2: typ) ->
       (p1: path from to1) ->
       (p2: path from to2 {path_includes p1 p2} ) ->
       GTot Type0)
   (h_step:
-    (#through: Type) ->
-    (#to: Type) ->
+    (#through: typ) ->
+    (#to: typ) ->
     (p: path from through) ->
     (s: step through to { path_includes p (PathStep through to p s) } ) ->
     Lemma (x p (PathStep through to p s)))
   (h_refl:
-    (#to: Type) ->
+    (#to: typ) ->
     (p: path from to {path_includes p p}) ->
     Lemma (x p p))
   (h_trans:
-    (#to1: Type) ->
-    (#to2: Type) ->
-    (#to3: Type) ->
+    (#to1: typ) ->
+    (#to2: typ) ->
+    (#to3: typ) ->
     (p1: path from to1) ->
     (p2: path from to2) ->
     (p3: path from to3 {path_includes p1 p2 /\ path_includes p2 p3 /\ path_includes p1 p3 /\ x p1 p2 /\ x p2 p3}) ->
     Lemma (x p1 p3))
-  (#to1: Type)
-  (#to2: Type)
+  (#to1: typ)
+  (#to2: typ)
   (p1: path from to1)
   (p2: path from to2 {path_includes p1 p2})
 : Lemma
@@ -301,16 +540,17 @@ private let rec path_includes_ind
     )
 
 private let rec path_length
-  (#from #to: Type)
+  (#from #to: typ)
   (p: path from to)
 : Tot nat
+  (decreases p)
 = match p with
   | PathBase -> 0
   | PathStep _ _ p' _ -> 1 + path_length p'
 
 private let path_includes_length
-  (#from: Type)
-  (#to1 #to2: Type)
+  (#from: typ)
+  (#to1 #to2: typ)
   (p1: path from to1)
   (p2: path from to2 {path_includes p1 p2})
 : Lemma
@@ -323,9 +563,9 @@ private let path_includes_length
     p1 p2
 
 private let path_includes_step_l
-  (#from: Type)
-  (#through: Type)
-  (#to: Type)
+  (#from: typ)
+  (#through: typ)
+  (#to: typ)
   (p: path from through)
   (s: step through to)
 : Lemma
@@ -336,9 +576,9 @@ private let path_includes_step_l
   FStar.Classical.forall_intro (path_includes_length #from #to #through (PathStep through to p s))
 
 private let rec path_includes_concat
-  (#from: Type)
-  (#through: Type)
-  (#to: Type)
+  (#from: typ)
+  (#through: typ)
+  (#to: typ)
   (p: path from through)
   (q: path through to)
 : Lemma
@@ -351,9 +591,9 @@ private let rec path_includes_concat
   | PathStep _ _ q' _ -> path_includes_concat p q'
 
 private let path_includes_exists_concat
-  (#from #through: Type)
+  (#from #through: typ)
   (p: path from through)
-  (#to: Type)
+  (#to: typ)
   (q: path from to { path_includes p q } )
 : Lemma
   (ensures (exists (r: path through to) . q == path_concat p r))
@@ -371,28 +611,50 @@ private let path_includes_exists_concat
     )
     p q
 
+private
 let step_disjoint
-  (#from: Type)
-  (#to1 #to2: Type)
+  (#from: typ)
+  (#to1 #to2: typ)
   (s1: step from to1)
   (s2: step from to2)
-: GTot Type0
+: GTot bool
 = match s1 with
-  | StepField key1 value1 fd1 ->
-    begin match s2 with
-    | StepField key2 value2 fd2 ->
-      key1 == key2 /\ value1 == value2 /\ fd1 <> fd2
-    | _ -> False
-    end
-  | StepCell length1 value1 i1 ->
-    begin match s2 with
-    | StepCell length2 value2 i2 -> length1 == length2 /\ value1 == value2 /\ UInt32.v i1 <> UInt32.v i2
-    | _ -> False
-    end
+  | StepField _ fd1 ->
+    let (StepField _ fd2) = s2 in
+    fd1 <> fd2
+  | StepCell _ _ i1 ->
+    let (StepCell _ _ i2) = s2 in
+    UInt32.v i1 <> UInt32.v i2
 
+private
+let step_eq
+  (#from: typ)
+  (#to1 #to2: typ)
+  (s1: step from to1)
+  (s2: step from to2)
+: Tot (b: bool { b = true <==> to1 == to2 /\ s1 == s2 } )
+= match s1 with
+  | StepField l1 fd1 ->
+    let (StepField _ fd2) = s2 in
+    fd1 = fd2
+  | StepCell _ _ i1 ->
+    let (StepCell _ _ i2) = s2 in
+    i1 = i2
+
+private
+let step_disjoint_not_eq
+  (#from: typ)
+  (#to1 #to2: typ)
+  (s1: step from to1)
+  (s2: step from to2)
+: Lemma
+  (ensures (step_disjoint s1 s2 = not (step_eq s1 s2)))
+= ()
+
+private
 let step_disjoint_sym
-  (#from: Type)
-  (#to1 #to2: Type)
+  (#from: typ)
+  (#to1 #to2: typ)
   (s1: step from to1)
   (s2: step from to2)
 : Lemma
@@ -400,65 +662,65 @@ let step_disjoint_sym
   (ensures (step_disjoint s2 s1))
 = ()
 
-noeq private type path_disjoint_t (#from: Type):
-  (#to1: Type) ->
-  (#to2: Type) ->
+noeq private type path_disjoint_t (#from: typ):
+  (#to1: typ) ->
+  (#to2: typ) ->
   (p1: path from to1) ->
   (p2: path from to2) ->
-  Type
+  Type0
 = | PathDisjointStep:
-    (#through: Type) ->
-    (#to1: Type) ->
-    (#to2: Type) ->
+    (#through: typ) ->
+    (#to1: typ) ->
+    (#to2: typ) ->
     (p: path from through) ->
     (s1: step through to1) ->
     (s2: step through to2 { step_disjoint s1 s2 } ) ->
     path_disjoint_t (PathStep through to1 p s1) (PathStep through to2 p s2)
   | PathDisjointIncludes:
-    (#to1: Type) ->
-    (#to2: Type) ->
+    (#to1: typ) ->
+    (#to2: typ) ->
     (p1: path from to1) ->
     (p2: path from to2) ->
-    (#to1': Type) ->
-    (#to2': Type) ->
+    (#to1': typ) ->
+    (#to2': typ) ->
     (p1': path from to1' {path_includes p1 p1'}) ->
     (p2': path from to2' {path_includes p2 p2'}) ->
     path_disjoint_t p1 p2 ->
     path_disjoint_t p1' p2'
 
 private let rec path_disjoint_t_rect
-  (#from: Type)
+  (#from: typ)
   (x:
-    (#value1: Type) ->
-    (#value2: Type) ->
+    (#value1: typ) ->
+    (#value2: typ) ->
     (p1: path from value1) ->
     (p2: path from value2) ->
     (h: path_disjoint_t p1 p2) ->
     GTot Type)
   (h_step:
-    (#through: Type) ->
-    (#to1: Type) ->
-    (#to2: Type) ->
+    (#through: typ) ->
+    (#to1: typ) ->
+    (#to2: typ) ->
     (p: path from through) ->
     (s1: step through to1) ->
     (s2: step through to2 { step_disjoint s1 s2 } ) ->
     (h: path_disjoint_t (PathStep through to1 p s1) (PathStep through to2 p s2)) ->
     GTot (x (PathStep through to1 p s1) (PathStep through to2 p s2) h))
   (h_includes:
-    (#value1: Type) ->
-    (#value2: Type) ->
+    (#value1: typ) ->
+    (#value2: typ) ->
     (p1: path from value1) ->
     (p2: path from value2) ->
-    (#value1': Type) ->
-    (#value2': Type) ->
+    (#value1': typ) ->
+    (#value2': typ) ->
     (p1': path from value1' {path_includes p1 p1'}) ->
     (p2': path from value2' {path_includes p2 p2'}) ->
     (h: path_disjoint_t p1 p2) ->
     (h': path_disjoint_t p1' p2') ->
     (ihx: x p1 p2 h) ->
     GTot (x p1' p2' h'))
-  (#value1: Type)
-  (#value2: Type)
+  (#value1: typ)
+  (#value2: typ)
   (p1: path from value1)
   (p2: path from value2)
   (h: path_disjoint_t p1 p2)
@@ -471,42 +733,42 @@ private let rec path_disjoint_t_rect
   | PathDisjointIncludes p1_ p2_ p1' p2' h_ -> h_includes p1_ p2_ p1' p2' h_ h (path_disjoint_t_rect x h_step h_includes p1_ p2_ h_)
 
 private let path_disjoint
-  (#from: Type)
-  (#value1: Type)
-  (#value2: Type)
+  (#from: typ)
+  (#value1: typ)
+  (#value2: typ)
   (p1: path from value1)
   (p2: path from value2)
 : GTot Type0
 = squash (path_disjoint_t p1 p2)
 
-abstract let path_disjoint_ind
-  (#from: Type)
+private let path_disjoint_ind
+  (#from: typ)
   (x:
-    (#value1: Type) ->
-    (#value2: Type) ->
+    (#value1: typ) ->
+    (#value2: typ) ->
     (p1: path from value1) ->
     (p2: path from value2 {path_disjoint p1 p2} ) ->
-    GTot Type0)
+    GTot Type)
   (h_step:
-    (#through: Type) ->
-    (#to1: Type) ->
-    (#to2: Type) ->
+    (#through: typ) ->
+    (#to1: typ) ->
+    (#to2: typ) ->
     (p: path from through) ->
     (s1: step through to1) ->
     (s2: step through to2 { step_disjoint s1 s2 /\ path_disjoint (PathStep through to1 p s1) (PathStep through to2 p s2) } ) ->
     Lemma (x (PathStep through to1 p s1) (PathStep through to2 p s2) ))
   (h_includes:
-    (#value1: Type) ->
-    (#value2: Type) ->
+    (#value1: typ) ->
+    (#value2: typ) ->
     (p1: path from value1) ->
     (p2: path from value2) ->
-    (#value1': Type) ->
-    (#value2': Type) ->
+    (#value1': typ) ->
+    (#value2': typ) ->
     (p1': path from value1' {path_includes p1 p1'}) ->
     (p2': path from value2' {path_includes p2 p2' /\ path_disjoint p1 p2 /\ path_disjoint p1' p2' /\ x p1 p2}) ->
     Lemma (x p1' p2'))
-  (#value1: Type)
-  (#value2: Type)
+  (#value1: typ)
+  (#value2: typ)
   (p1: path from value1)
   (p2: path from value2 { path_disjoint p1 p2 } )
 : Lemma (x p1 p2)
@@ -523,10 +785,10 @@ abstract let path_disjoint_ind
      p1 p2 h)
 
 private let path_disjoint_step
-  (#from: Type)
-  (#through: Type)
-  (#to1: Type)
-  (#to2: Type)
+  (#from: typ)
+  (#through: typ)
+  (#to1: typ)
+  (#to2: typ)
   (p: path from through)
   (s1: step through to1)
   (s2: step through to2 { step_disjoint s1 s2 } )
@@ -537,13 +799,13 @@ private let path_disjoint_step
 = FStar.Squash.return_squash (PathDisjointStep p s1 s2)
 
 private let path_disjoint_includes
-  (#from: Type)
-  (#to1: Type)
-  (#to2: Type)
+  (#from: typ)
+  (#to1: typ)
+  (#to2: typ)
   (p1: path from to1)
   (p2: path from to2)
-  (#to1': Type)
-  (#to2': Type)
+  (#to1': typ)
+  (#to2': typ)
   (p1': path from to1')
   (p2': path from to2' {path_disjoint p1 p2 /\ path_includes p1 p1' /\ path_includes p2 p2'} )
 : Lemma
@@ -551,10 +813,11 @@ private let path_disjoint_includes
 = let h : squash (path_disjoint_t p1 p2) = FStar.Squash.join_squash () in
   FStar.Squash.bind_squash h (fun h -> FStar.Squash.return_squash (PathDisjointIncludes p1 p2 p1' p2' h))
 
+private
 let rec path_disjoint_sym
-  (#from: Type)
-  (#value1: Type)
-  (#value2: Type)
+  (#from: typ)
+  (#value1: typ)
+  (#value2: typ)
   (p1: path from value1)
   (p2: path from value2)
 : Lemma
@@ -566,23 +829,295 @@ let rec path_disjoint_sym
   (fun #v1 #v2 p1 p2 #v1' #v2' p1' p2' -> path_disjoint_includes p2 p1 p2' p1')
   p1 p2
 
+private let rec path_equal
+  (#from: typ)
+  (#value1: typ)
+  (#value2: typ)
+  (p1: path from value1)
+  (p2: path from value2)
+: Tot (b: bool { b == true <==> (value1 == value2 /\ p1 == p2) } )
+  (decreases p1)
+= match p1 with
+  | PathBase -> PathBase? p2
+  | PathStep _ _ p1' s1 ->
+    PathStep? p2 && (
+      let (PathStep _ _ p2' s2) = p2 in (
+        path_equal p1' p2' &&
+        step_eq s1 s2
+    ))
+
+private
+let rec path_length_concat
+  (#t0 #t1 #t2: typ)
+  (p01: path t0 t1)
+  (p12: path t1 t2)
+: Lemma
+  (requires True)
+  (ensures (path_length (path_concat p01 p12) == path_length p01 + path_length p12))
+  (decreases p12)
+= match p12 with
+  | PathBase -> ()
+  | PathStep _ _ p' s' -> path_length_concat p01 p'
+
+private
+let rec path_concat_inj_l
+  (#from #through1: typ)
+  (p1_: path from through1)
+  (#v1: typ)
+  (p1: path through1 v1)
+  (#through2 #v2: typ)
+  (p2_: path from through2)
+  (p2: path through2 v2)
+: Lemma
+  (requires (path_equal (path_concat p1_ p1) (path_concat p2_ p2) == true /\ path_length p1_ == path_length p2_))
+  (ensures (path_equal p1_ p2_ == true /\ path_equal p1 p2 == true))
+  (decreases p1)
+= path_length_concat p1_ p1;
+  path_length_concat p2_ p2;
+  match p1 with
+  | PathBase -> ()
+  | PathStep _ _ p1' s1 ->
+    let (PathStep _ _ p2' s2) = p2 in
+    path_concat_inj_l p1_ p1' p2_ p2'
+
+private type path_disjoint_decomp_t
+  (#from: typ)
+  (#value1: typ)
+  (#value2: typ)
+  (p1: path from value1)
+  (p2: path from value2)
+: Type
+= | PathDisjointDecomp:
+    (d_through: typ) ->
+    (d_p: path from d_through) ->
+    (d_v1: typ) ->
+    (d_s1: step d_through d_v1) ->
+    (d_p1': path d_v1 value1) ->
+    (d_v2: typ) ->
+    (d_s2: step d_through d_v2) ->
+    (d_p2': path d_v2 value2) ->
+    squash (
+      step_eq d_s1 d_s2 == false /\
+      p1 == path_concat (PathStep _ _ d_p d_s1) d_p1' /\
+      p2 == path_concat (PathStep _ _ d_p d_s2) d_p2'
+    ) ->
+    path_disjoint_decomp_t p1 p2
+
+#reset-options "--z3rlimit 16"
+
+private let path_disjoint_decomp_includes
+  (#from: typ)
+  (#value1: typ)
+  (#value2: typ)
+  (p1: path from value1)
+  (p2: path from value2)
+  (#value1': typ)
+  (#value2': typ)
+  (p1': path from value1')
+  (p2': path from value2')
+: Lemma
+  (requires (
+    path_includes p1 p1' /\
+    path_includes p2 p2' /\ (
+    exists (d : path_disjoint_decomp_t p1 p2) . True
+  )))
+  (ensures (exists (d: path_disjoint_decomp_t p1' p2') . True))
+= let f
+    (q1: path value1 value1' )
+    (q2: path value2 value2' )
+    (d: path_disjoint_decomp_t p1 p2)
+  : Lemma
+    (requires (
+      p1' == path_concat p1 q1 /\
+      p2' == path_concat p2 q2
+    ))
+    (ensures (exists (d: path_disjoint_decomp_t p1' p2') . True))
+  = let (PathDisjointDecomp _ p _ s1 p1_ _ s2 p2_ _) = d in
+    path_concat_assoc (PathStep _ _ p s1) p1_ q1;
+    path_concat_assoc (PathStep _ _ p s2) p2_ q2;
+    let d' : path_disjoint_decomp_t p1' p2' =
+      PathDisjointDecomp _ p _ s1 (path_concat p1_ q1) _ s2 (path_concat p2_ q2) ()
+    in
+    Classical.exists_intro (fun _ -> True) d'
+  in
+  let g
+    (q1: path value1 value1' )
+    (q2: path value2 value2' )
+    (d: path_disjoint_decomp_t p1 p2)
+  : Lemma
+    ((
+      p1' == path_concat p1 q1 /\
+      p2' == path_concat p2 q2
+    ) ==> (
+      exists (d: path_disjoint_decomp_t p1' p2') . True
+    ))
+  = Classical.move_requires (f q1 q2) d // FIXME: annoying to repeat those type annotations above. WHY WHY WHY can't I just use (fun q1 q2 d -> Classical.move_requires (f q1 q2) d) as an argument of Classical.forall_intro_3 below instead of this g???
+  in  
+  path_includes_exists_concat p1 p1' ;
+  path_includes_exists_concat p2 p2' ;
+  let _ : squash (exists (d: path_disjoint_decomp_t p1' p2') . True) =
+    Classical.forall_intro_3 g
+  in
+  ()
+
+private
+let path_disjoint_decomp
+  (#from: typ)
+  (#value1: typ)
+  (#value2: typ)
+  (p1: path from value1)
+  (p2: path from value2)
+: Lemma
+  (requires (path_disjoint p1 p2))
+  (ensures (exists (d: path_disjoint_decomp_t p1 p2) . True))
+= path_disjoint_ind
+  (fun #v1 #v2 p1 p2 -> exists (d: path_disjoint_decomp_t p1 p2) . True)
+  (fun #through #to1 #to2 p s1 s2 ->
+    let d : path_disjoint_decomp_t (PathStep _ _ p s1) (PathStep _ _ p s2) =
+      PathDisjointDecomp _ p _ s1 PathBase _ s2 PathBase ()
+    in
+    Classical.exists_intro (fun _ -> True) d
+  )
+  (fun #v1 #v2 p1 p2 #v1' #v2' p1' p2' -> path_disjoint_decomp_includes p1 p2 p1' p2')
+  p1 p2
+
+private
+let path_disjoint_not_path_equal
+  (#from: typ)
+  (#value1: typ)
+  (#value2: typ)
+  (p1: path from value1)
+  (p2: path from value2)
+: Lemma
+  (requires (path_disjoint p1 p2))
+  (ensures (path_equal p1 p2 == false))
+= let f
+    (d: path_disjoint_decomp_t p1 p2)
+  : Lemma (path_equal p1 p2 == false)
+  = if path_equal p1 p2
+    then
+      let (PathDisjointDecomp _ p _ s1 p1_ _ s2 p2_ _) = d in
+      path_concat_inj_l (PathStep _ _ p s1) p1_ (PathStep _ _ p s2) p2_
+    else ()
+  in
+  path_disjoint_decomp p1 p2;
+  Classical.forall_intro f
+
+private
+let rec path_destruct_l
+  (#t0 #t2: typ)
+  (p: path t0 t2)
+: Tot (
+    x: option (t1: typ & (s: step t0 t1 & (p' : path t1 t2 { p == path_concat (PathStep _ _ PathBase s) p' /\ path_length p' < path_length p } ) ) )
+    { None? x <==> PathBase? p }
+  )
+  (decreases p)
+= match p with
+  | PathBase -> None
+  | PathStep _ _ p' s ->
+    begin match path_destruct_l p' with
+    | None -> Some (| _, (| s,  PathBase |) |)
+    | Some (| t_, (| s_, p_ |) |) ->
+      Some (| t_, (| s_, PathStep _ _ p_ s |) |)
+    end
+
+private
+let rec path_equal'
+  (#from #to1 #to2: typ)
+  (p1: path from to1)
+  (p2: path from to2)
+: Tot (b: bool { b == true <==> to1 == to2 /\ p1 == p2 } )
+  (decreases (path_length p1))
+= match path_destruct_l p1 with
+  | None -> PathBase? p2
+  | Some (| t1, (| s1, p1' |) |) ->
+    begin match path_destruct_l p2 with
+    | None -> false
+    | (Some (| t2, (| s2, p2' |) |) ) ->
+      step_eq s1 s2 &&
+      path_equal' p1' p2'
+    end
+
+private
+let path_includes_concat_l
+  (#from #through #to1 #to2: typ)
+  (p0: path from through)
+  (p1: path through to1)
+  (p2: path through to2)
+: Lemma
+  (requires (path_includes p1 p2))
+  (ensures (path_includes (path_concat p0 p1) (path_concat p0 p2)))
+= path_includes_ind
+    (fun #to1_ #to2_ p1_ p2_ -> path_includes (path_concat p0 p1_) (path_concat p0 p2_))
+    (fun #through #to p st -> ())
+    (fun #to p -> path_includes_refl (path_concat p0 p))
+    (fun #to1_ #to2_ #to3_ p1_ p2_ p3_ -> path_includes_trans (path_concat p0 p1_) (path_concat p0 p2_) (path_concat p0 p3_))
+    p1 p2
+
+private
+let path_disjoint_concat
+  (#from #through #to1 #to2: typ)
+  (p0: path from through)
+  (p1: path through to1)
+  (p2: path through to2)
+: Lemma
+  (requires (path_disjoint p1 p2))
+  (ensures (path_disjoint (path_concat p0 p1) (path_concat p0 p2)))
+= path_disjoint_ind
+    (fun #v1 #v2 p1 p2 -> path_disjoint (path_concat p0 p1) (path_concat p0 p2))
+    (fun #through #to1 #to2 p s1 s2 -> path_disjoint_step (path_concat p0 p) s1 s2)
+    (fun #v1 #v2 p1 p2 #v1' #v2' p1' p2' ->
+      path_includes_concat_l p0 p1 p1';
+      path_includes_concat_l p0 p2 p2';
+      path_disjoint_includes (path_concat p0 p1) (path_concat p0 p2) (path_concat p0 p1') (path_concat p0 p2'))
+  p1 p2
+
+private
+let rec not_path_equal_path_disjoint_same_type
+  (#from: typ)
+  (#value: typ)
+  (p1: path from value)
+  (p2: path from value)
+: Lemma
+  (requires (path_equal p1 p2 == false))
+  (ensures (path_disjoint p1 p2))
+  (decreases (path_length p1))
+= assert (path_equal p1 p2 == path_equal' p1 p2);
+  match path_destruct_l p1 with
+  | None -> path_typ_depth p2
+  | Some (| t1, (| s1, p1' |) |) ->
+    begin match path_destruct_l p2 with
+    | None -> path_typ_depth p1
+    | Some (| t2, (| s2, p2' |) |) ->
+      if step_eq s1 s2
+      then begin
+	not_path_equal_path_disjoint_same_type p1' p2' ;
+	path_disjoint_concat (PathStep _ _ PathBase s1) p1' p2'
+      end else begin
+        path_disjoint_step PathBase s1 s2;
+	path_includes_concat (PathStep _ _ PathBase s1) p1';
+	path_includes_concat (PathStep _ _ PathBase s2) p2';
+	path_disjoint_includes (PathStep _ _ PathBase s1) (PathStep _ _ PathBase s2) p1 p2
+      end
+    end
+
 private let path_sel_upd_other
-  (#from: Type)
-  (#to1 #to2: Type)
+  (#from: typ)
+  (#to1 #to2: typ)
   (p1: path from to1)
   (p2: path from to2 {path_disjoint p1 p2})
 : Lemma
-  (ensures (forall (m: from) (v: to1) . path_sel (path_upd m p1 v) p2 == path_sel m p2))
+  (ensures (forall (m: type_of_typ from) (v: type_of_typ to1) . path_sel (path_upd m p1 v) p2 == path_sel m p2))
 = path_disjoint_ind
-  (fun #v1 #v2 p1_ p2_ -> forall (m: from) (v: v1) . path_sel (path_upd m p1_ v) p2_ == path_sel m p2_)
+  (fun #v1 #v2 p1_ p2_ -> forall (m: type_of_typ from) (v: type_of_typ v1) . path_sel (path_upd m p1_ v) p2_ == path_sel m p2_)
   (fun #through #to1_ #to2_ p s1 s2 ->
-      FStar.Classical.forall_intro' #_ #(fun m -> forall  (v: to1_) . path_sel (path_upd m (PathStep through to1_ p s1) v) (PathStep through to2_ p s2) == path_sel m (PathStep through to2_ p s2)) (fun m ->
+      FStar.Classical.forall_intro' #_ #(fun m -> forall  (v: type_of_typ to1_) . path_sel (path_upd m (PathStep through to1_ p s1) v) (PathStep through to2_ p s2) == path_sel m (PathStep through to2_ p s2)) (fun m ->
 	  FStar.Classical.forall_intro' #_ #(fun v -> path_sel (path_upd m (PathStep through to1_ p s1) v) (PathStep through to2_ p s2) == path_sel m (PathStep through to2_ p s2)) (fun v ->
 	  match s1 with
-	  | StepField key1 value1 fd1 ->
-	    let (StepField _ _ fd2) = s2 in
-	    let (s: DM.t key1 value1) = path_sel m p in
-	    path_sel_upd_same m p (DM.upd s fd1 v);
+	  | StepField l1 fd1 ->
+	    let (StepField _ fd2) = s2 in
+	    let (s: struct l1) = path_sel m p in
+	    path_sel_upd_same m p (struct_upd s fd1 v);
 	    DM.sel_upd_other s fd1 v fd2
 	  | StepCell length1 value1 i1 ->
 	    let (StepCell _ _ i2) = s2 in
@@ -592,8 +1127,8 @@ private let path_sel_upd_other
   (fun #v1 #v2 p1 p2 #v1' #v2' p1' p2' ->
     let h1: squash (exists r1 . p1' == path_concat p1 r1) = path_includes_exists_concat p1 p1' in
     let h2: squash (exists r2 . p2' == path_concat p2 r2) = path_includes_exists_concat p2 p2' in
-    FStar.Classical.forall_intro' #_ #(fun (m: from) -> forall v . path_sel (path_upd m p1' v) p2' == path_sel m p2') (fun (m: from) ->
-      FStar.Classical.forall_intro' #_ #(fun (v: v1') -> path_sel (path_upd m p1' v) p2' == path_sel m p2') (fun (v: v1') ->
+    FStar.Classical.forall_intro' #_ #(fun (m: type_of_typ from) -> forall v . path_sel (path_upd m p1' v) p2' == path_sel m p2') (fun (m: type_of_typ from) ->
+      FStar.Classical.forall_intro' #_ #(fun (v: type_of_typ v1') -> path_sel (path_upd m p1' v) p2' == path_sel m p2') (fun (v: type_of_typ v1') ->
       FStar.Classical.exists_elim (path_sel (path_upd m p1' v) p2' == path_sel m p2') h1 (fun r1 ->
 	FStar.Classical.exists_elim (path_sel (path_upd m p1' v) p2' == path_sel m p2') h2 (fun r2 ->
 	  path_upd_concat m p1 r1 v;
@@ -602,163 +1137,218 @@ private let path_sel_upd_other
   p1 p2
 
 private let path_sel_upd_other'
-  (#from: Type)
-  (#to1 #to2: Type)
+  (#from: typ)
+  (#to1 #to2: typ)
   (p1: path from to1)
   (p2: path from to2 {path_disjoint p1 p2})
-  (m: from)
-  (v: to1)
+  (m: type_of_typ from)
+  (v: type_of_typ to1)
 : Lemma
   (requires True)
   (ensures (path_sel (path_upd m p1 v) p2 == path_sel m p2))
   [SMTPat (path_sel (path_upd m p1 v) p2)]
 = path_sel_upd_other p1 p2
 
-(** Pointers to data of type t *)
+(* Pointers *)
 
-noeq private type _pointer : Type -> Tot Type =
-  | Pointer:
-    (#from: Type) ->
-    (content: HS.reference from ) ->
-    (#to: Type) ->
-    (p: path from to) ->
-    _pointer to
-abstract let pointer (t: Type): Tot Type =
-  _pointer t
+abstract let equal
+  (#t1 #t2: typ)
+  (p1: pointer t1)
+  (p2: pointer t2)
+: Ghost bool
+  (requires True)
+  (ensures (fun b -> b == true <==> t1 == t2 /\ p1 == p2 ))
+= Pointer?.from p1 = Pointer?.from p2 &&
+  HS.aref_equal (Pointer?.contents p1) (Pointer?.contents p2) &&
+  path_equal p1.p p2.p
 
-abstract let as_addr (#t: Type) (p: pointer t): GTot nat =
-  HS.as_addr (Pointer?.content p)
+abstract let as_addr (#t: typ) (p: pointer t): GTot nat =
+  HS.aref_as_addr (Pointer?.contents p)
 
 private let _field
-  (#key: eqtype)
-  (#value: (key -> Tot Type))
-  (p: pointer (DM.t key value))
-  (fd: key)
-: Tot (pointer (value fd))
-= let (Pointer #from content p') = p in
-  let p' : path from (DM.t key value) = p' in
-  let p'' : path from (value fd) = PathStep _ _ p' (StepField _ _ fd) in
-  Pointer content p''
+  (#l: struct_typ)
+  (p: pointer (TStruct l))
+  (fd: struct_field l)
+: Tot (pointer (typ_of_struct_field l fd))
+= let (Pointer from contents p') = p in
+  let p' : path from (TStruct l) = p' in
+  let p'' : path from (typ_of_struct_field l fd) = PathStep _ _ p' (StepField _ fd) in
+  Pointer from contents p''
 
 private let _cell
   (#length: UInt32.t)
-  (#value: Type)
-  (p: pointer (array length value))
+  (#value: typ)
+  (p: pointer (TArray length value))
   (i: UInt32.t {UInt32.v i < UInt32.v length})
 : Tot (pointer value)
-= let (Pointer #from content p') = p in
-  let p' : path from (array length value) = p' in
+= let (Pointer from contents p') = p in
+  let p' : path from (TArray length value) = p' in
   let p'' : path from value = PathStep _ _ p' (StepCell _ _ i) in
-  Pointer content p''
+  Pointer from contents p''
 
 abstract let unused_in
-  (#value: Type)
+  (#value: typ)
   (p: pointer value)
   (h: HS.mem)
 : GTot Type0
-= HS.unused_in (Pointer?.content p) h
+= let (Pointer from contents p') = p in
+  HS.aref_unused_in contents h
+
+private
+let pointer_ref_contents : Type0 = (t: typ & type_of_typ t)
 
 abstract let live
-  (#value: Type)
+  (#value: typ)
   (h: HS.mem)
   (p: pointer value)
 : GTot Type0
-= HS.contains h (Pointer?.content p)
+= let (Pointer from contents _) = p in (
+    HS.aref_live_at h contents pointer_ref_contents /\ (
+      let untyped_contents = HS.greference_of contents pointer_ref_contents in (
+      dfst (HS.sel h untyped_contents) == from
+  )))
+
+private let greference_of
+  (#value: typ)
+  (p: pointer value)
+: Ghost (HS.reference pointer_ref_contents)
+  (requires (exists h . live h p))
+  (ensures (fun x -> (exists h . live h p) /\ x == HS.greference_of (Pointer?.contents p) pointer_ref_contents /\ HS.aref_of x == Pointer?.contents p))
+= HS.greference_of (Pointer?.contents p) pointer_ref_contents
+
+private
+let reference_of
+  (h: HS.mem)
+  (#value: typ)
+  (p: pointer value)
+: Pure (HS.reference pointer_ref_contents)
+  (requires (live h p))
+  (ensures (fun x -> live h p /\ x == greference_of p))
+= HS.reference_of h (Pointer?.contents p) pointer_ref_contents
+
+private
+let unused_in_greference_of
+  (#value: typ)
+  (p: pointer value)
+  (h: HS.mem)
+: Lemma
+  (requires (exists h . live h p))
+  (ensures ((exists h . live h p) /\ (HS.unused_in (greference_of p) h <==> unused_in p h)))
+  [SMTPatOr [
+    [SMTPat (HS.unused_in (greference_of p) h)];
+    [SMTPat (unused_in p h)];
+  ]]
+= ()
 
 abstract let live_not_unused_in
-  (#value: Type)
+  (#value: typ)
   (h: HS.mem)
   (p: pointer value)
 : Lemma
   (ensures (live h p /\ p `unused_in` h ==> False))
   [SMTPatT (live h p); SMTPatT (p `unused_in` h)]
-= ()
+= let f () : Lemma
+    (requires (live h p /\ p `unused_in` h))
+    (ensures False)
+  = let r = greference_of p in
+    HS.contains_aref_unused_in h r (Pointer?.contents p)
+  in
+  Classical.move_requires f ()
 
 abstract let gread
-  (#value: Type)
+  (#value: typ)
   (h: HS.mem)
   (p: pointer value)
-: GTot value
-= let (Pointer content p') = p in
-  path_sel (HS.sel h content) p'
+: GTot (type_of_typ value)
+= if StrongExcludedMiddle.strong_excluded_middle (live h p)
+  then
+    let content = greference_of p in
+    let (| _, c |) = HS.sel h content in
+    path_sel c p.p
+  else
+    dummy_val value
 
 abstract let frameOf
-  (#value: Type)
+  (#value: typ)
   (p: pointer value)
 : GTot HH.rid
-= HS.frameOf (Pointer?.content p)
+= HS.frameOf_aref (Pointer?.contents p)
 
 abstract let disjoint_roots_intro_pointer_vs_pointer
-  (#value1 value2: Type)
+  (#value1 value2: typ)
   (h: HS.mem)
   (p1: pointer value1)
   (p2: pointer value2)
 : Lemma
   (requires (live h p1 /\ unused_in p2 h))
   (ensures (frameOf p1 <> frameOf p2 \/ as_addr p1 =!= as_addr p2))
-= HyperStack.lemma_live_1 h (Pointer?.content p1) (Pointer?.content p2)
+= ()
 
 abstract let disjoint_roots_intro_pointer_vs_reference
-  (#value1 value2: Type)
+  (#value1: typ)
+  (#value2: Type)
   (h: HS.mem)
   (p1: pointer value1)
   (p2: HS.reference value2)
 : Lemma
   (requires (live h p1 /\ p2 `HS.unused_in` h))
   (ensures (frameOf p1 <> HS.frameOf p2 \/ as_addr p1 =!= HS.as_addr p2))
-= HyperStack.lemma_live_1 h (Pointer?.content p1) p2
+= ()
 
 abstract let disjoint_roots_intro_reference_vs_pointer
-  (#value1 value2: Type)
+  (#value1: Type)
+  (#value2: typ)
   (h: HS.mem)
   (p1: HS.reference value1)
   (p2: pointer value2)
 : Lemma
   (requires (HS.contains h p1 /\ p2 `unused_in` h))
   (ensures (HS.frameOf p1 <> frameOf p2 \/ HS.as_addr p1 =!= as_addr p2))
-= HyperStack.lemma_live_1 h p1 (Pointer?.content p2)
+= ()
 
-let memory_managed
-  (#value: Type)
+abstract let is_mm
+  (#value: typ)
   (p: pointer value)
 : GTot bool
-= HS.is_mm (Pointer?.content p)
+= HS.aref_is_mm (Pointer?.contents p)
 
+(* // TODO: recover with addresses?
 abstract let recall
   (#value: Type)
-  (p: pointer value {HS.is_eternal_region (frameOf p) && not (memory_managed p)})
+  (p: pointer value {HS.is_eternal_region (frameOf p) && not (is_mm p)})
 : HST.Stack unit
   (requires (fun m -> True))
   (ensures (fun m0 _ m1 -> m0 == m1 /\ live m1 p))
 = HST.recall (Pointer?.content p)
+*)
 
 (* Equality predicate on struct contents, without quantifiers *)
 let equal_values #a h (b:pointer a) h' (b':pointer a) : GTot Type0 =
   live h b /\ live h' b' /\ gread h b == gread h' b'
 
 abstract let includes
-  (#value1: Type)
-  (#value2: Type)
+  (#value1: typ)
+  (#value2: typ)
   (p1: pointer value1)
   (p2: pointer value2)
-: GTot Type0
-= Pointer?.from p1 == Pointer?.from p2 /\ Pointer?.content p1 == Pointer?.content p2 /\ path_includes (Pointer?.p p1) (Pointer?.p p2)
+: GTot bool
+= Pointer?.from p1 = Pointer?.from p2 &&
+  HS.aref_equal (Pointer?.contents p1) (Pointer?.contents p2) &&
+  path_includes (Pointer?.p p1) (Pointer?.p p2)
 
 #reset-options "--z3rlimit 16"
 
 abstract let gfield
-  (#key: eqtype)
-  (#value: (key -> Tot Type))
-  (p: pointer (DM.t key value))
-  (fd: key)
-: GTot (p' : pointer (value fd) { includes p p' } )
+  (#l: struct_typ)
+  (p: pointer (TStruct l))
+  (fd: struct_field l)
+: GTot (p' : pointer (typ_of_struct_field l fd) { includes p p' } )
 = _field p fd
 
 abstract let as_addr_gfield
-  (#key: eqtype)
-  (#value: (key -> Tot Type))
-  (p: (pointer (DM.t key value)))
-  (fd: key)
+  (#l: struct_typ)
+  (p: pointer (TStruct l))
+  (fd: struct_field l)
 : Lemma
   (requires True)
   (ensures (as_addr (gfield p fd) == as_addr p))
@@ -766,11 +1356,10 @@ abstract let as_addr_gfield
 = ()
 
 abstract let unused_in_gfield
-  (#key: eqtype)
-  (#value: (key -> Tot Type))
+  (#l: struct_typ)
+  (p: pointer (TStruct l))
+  (fd: struct_field l)
   (h: HS.mem)
-  (p: (pointer (DM.t key value)))
-  (fd: key)
 : Lemma
   (requires True)
   (ensures (unused_in (gfield p fd) h <==> unused_in p h))
@@ -778,11 +1367,10 @@ abstract let unused_in_gfield
 = ()
 
 abstract let live_gfield
-  (#key: eqtype)
-  (#value: (key -> Tot Type))
   (h: HS.mem)
-  (p: pointer (DM.t key value))
-  (fd: key)
+  (#l: struct_typ)
+  (p: pointer (TStruct l))
+  (fd: struct_field l)
 : Lemma
   (requires True)
   (ensures (live h (gfield p fd) <==> live h p))
@@ -790,44 +1378,40 @@ abstract let live_gfield
 = ()
 
 abstract let gread_gfield
-  (#key: eqtype)
-  (#value: (key -> Tot Type))
   (h: HS.mem)
-  (p: pointer (DM.t key value))
-  (fd: key)
+  (#l: struct_typ)
+  (p: pointer (TStruct l))
+  (fd: struct_field l)
 : Lemma
   (requires True)
-  (ensures (gread h (gfield p fd) == DM.sel (gread h p) fd))
-  [SMTPatOr [[SMTPat (gread h (gfield p fd))]; [SMTPat (DM.sel (gread h p) fd)]]]
+  (ensures (gread h (gfield p fd) == struct_sel (gread h p) fd))
+  [SMTPatOr [[SMTPat (gread h (gfield p fd))]; [SMTPat (struct_sel (gread h p) fd)]]]
 = ()
 
 abstract let frameOf_gfield
-  (#key: eqtype)
-  (#value: (key -> Tot Type))
-  (p: pointer (DM.t key value))
-  (fd: key)
+  (#l: struct_typ)
+  (p: pointer (TStruct l))
+  (fd: struct_field l)
 : Lemma
   (requires True)
   (ensures (frameOf (gfield p fd) == frameOf p))
   [SMTPat (frameOf (gfield p fd))]
 = ()
 
-abstract let memory_managed_gfield
-  (#key: eqtype)
-  (#value: (key -> Tot Type))
-  (p: pointer (DM.t key value))
-  (fd: key)
+abstract let is_mm_gfield
+  (#l: struct_typ)
+  (p: pointer (TStruct l))
+  (fd: struct_field l)
 : Lemma
   (requires True)
-  (ensures (memory_managed (gfield p fd) <==> memory_managed p))
-  [SMTPat (memory_managed (gfield p fd))]
+  (ensures (is_mm (gfield p fd) <==> is_mm p))
+  [SMTPat (is_mm (gfield p fd))]
 = ()
 
 abstract let includes_gfield
-  (#key: eqtype)
-  (#value: (key -> Tot Type))
-  (p: pointer (DM.t key value))
-  (fd: key)
+  (#l: struct_typ)
+  (p: pointer (TStruct l))
+  (fd: struct_field l)
 : Lemma
   (requires True)
   (ensures (includes p (gfield p fd)))
@@ -836,16 +1420,16 @@ abstract let includes_gfield
 
 abstract let gcell
   (#length: UInt32.t)
-  (#value: Type)
-  (p: pointer (array length value))
+  (#value: typ)
+  (p: pointer (TArray length value))
   (i: UInt32.t {UInt32.v i < UInt32.v length})
-: Tot (pointer value)
+: GTot (pointer value)
 = _cell p i
 
 abstract let as_addr_gcell
   (#length: UInt32.t)
-  (#value: Type)
-  (p: pointer (array length value))
+  (#value: typ)
+  (p: pointer (TArray length value))
   (i: UInt32.t {UInt32.v i < UInt32.v length})
 : Lemma
   (requires True)
@@ -855,9 +1439,9 @@ abstract let as_addr_gcell
 
 abstract let unused_in_gcell
   (#length: UInt32.t)
-  (#value: Type)
+  (#value: typ)
   (h: HS.mem)
-  (p: pointer (array length value))
+  (p: pointer (TArray length value))
   (i: UInt32.t {UInt32.v i < UInt32.v length})
 : Lemma
   (requires True)
@@ -867,9 +1451,9 @@ abstract let unused_in_gcell
 
 abstract let live_gcell
   (#length: UInt32.t)
-  (#value: Type)
+  (#value: typ)
   (h: HS.mem)
-  (p: pointer (array length value))
+  (p: pointer (TArray length value))
   (i: UInt32.t {UInt32.v i < UInt32.v length})
 : Lemma
   (requires True)
@@ -879,9 +1463,9 @@ abstract let live_gcell
 
 abstract let gread_gcell
   (#length: UInt32.t)
-  (#value: Type)
+  (#value: typ)
   (h: HS.mem)
-  (p: pointer (array length value))
+  (p: pointer (TArray length value))
   (i: UInt32.t {UInt32.v i < UInt32.v length})
 : Lemma
   (requires True)
@@ -891,8 +1475,8 @@ abstract let gread_gcell
 
 abstract let frameOf_gcell
   (#length: UInt32.t)
-  (#value: Type)
-  (p: pointer (array length value))
+  (#value: typ)
+  (p: pointer (TArray length value))
   (i: UInt32.t {UInt32.v i < UInt32.v length})
 : Lemma
   (requires True)
@@ -900,21 +1484,21 @@ abstract let frameOf_gcell
   [SMTPat (frameOf (gcell p i))]
 = ()
 
-abstract let memory_managed_gcell
+abstract let is_mm_gcell
   (#length: UInt32.t)
-  (#value: Type)
-  (p: pointer (array length value))
+  (#value: typ)
+  (p: pointer (TArray length value))
   (i: UInt32.t {UInt32.v i < UInt32.v length})
 : Lemma
   (requires True)
-  (ensures (memory_managed (gcell p i) == memory_managed p))
-  [SMTPat (memory_managed (gcell p i))]
+  (ensures (is_mm (gcell p i) == is_mm p))
+  [SMTPat (is_mm (gcell p i))]
 = ()
 
 abstract let includes_gcell
   (#length: UInt32.t)
-  (#value: Type)
-  (p: pointer (array length value))
+  (#value: typ)
+  (p: pointer (TArray length value))
   (i: UInt32.t {UInt32.v i < UInt32.v length})
 : Lemma
   (requires True)
@@ -923,7 +1507,7 @@ abstract let includes_gcell
 = ()
 
 abstract let includes_refl
-  (#value: Type)
+  (#value: typ)
   (p: pointer value)
 : Lemma
   (requires True)
@@ -932,7 +1516,7 @@ abstract let includes_refl
 = ()
 
 abstract let includes_trans
-  (#value1 #value2 #value3: Type)
+  (#value1 #value2 #value3: typ)
   (p1: pointer value1)
   (p2: pointer value2)
   (p3: pointer value3)
@@ -943,57 +1527,56 @@ abstract let includes_trans
 = path_includes_trans (Pointer?.p p1) (Pointer?.p p2) (Pointer?.p p3)
 
 abstract let includes_ind
-  (x: (#value1: Type) ->
-      (#value2: Type) ->
+  (x: (#value1: typ) ->
+      (#value2: typ) ->
       (p1: pointer value1) ->
       (p2: pointer value2 {includes p1 p2} ) ->
       GTot Type0)
   (h_field:
-    (#key: eqtype) ->
-    (#value: (key -> Tot Type)) ->
-    (p: pointer (DM.t key value)) ->
-    (fd: key {includes p (gfield p fd)}) ->
+    (l: struct_typ) ->
+    (p: pointer (TStruct l)) ->
+    (fd: struct_field l {includes p (gfield p fd)}) ->
     Lemma (x p (gfield p fd)))
   (h_cell:
     (#length: UInt32.t) ->
-    (#value: Type) ->
-    (p: pointer (array length value)) ->
+    (#value: typ) ->
+    (p: pointer (TArray length value)) ->
     (i: UInt32.t {UInt32.v i < UInt32.v length /\ includes p (gcell p i)}) ->
     Lemma (x p (gcell p i)))
   (h_refl:
-    (#value: Type) ->
+    (#value: typ) ->
     (p: pointer value {includes p p}) ->
     Lemma (x p p))
   (h_trans:
-    (#value1: Type) ->
-    (#value2: Type) ->
-    (#value3: Type) ->
+    (#value1: typ) ->
+    (#value2: typ) ->
+    (#value3: typ) ->
     (p1: pointer value1) ->
     (p2: pointer value2) ->
     (p3: pointer value3 {includes p1 p2 /\ includes p2 p3 /\ includes p1 p3 /\ x p1 p2 /\ x p2 p3}) ->
     Lemma (x p1 p3))
-  (#value1: Type)
-  (#value2: Type)
+  (#value1: typ)
+  (#value2: typ)
   (p1: pointer value1)
   (p2: pointer value2 {includes p1 p2})
 : Lemma (x p1 p2)
-= let from : Type = Pointer?.from p1 in
-  let content : HS.reference from = Pointer?.content p1 in
+= let (Pointer from contents _) = p1 in
   path_includes_ind
-    (fun #to1 #to2 p1_ p2_ -> x (Pointer content p1_) (Pointer content p2_))
+    (fun #to1 #to2 p1_ p2_ -> x (Pointer from contents p1_) (Pointer from contents p2_))
     (fun #through #to p s ->
       match s with
-      | StepField key value fd -> let (pt: pointer (DM.t key value)) = (Pointer content p) in h_field pt fd
-      | StepCell length value i -> let (pt: pointer (array length value)) = (Pointer content p) in h_cell pt i
+      | StepField l fd -> let (pt: pointer (TStruct l)) = (Pointer from contents p) in h_field l pt fd
+      | StepCell length value i -> let (pt: pointer (TArray length value)) = (Pointer from contents p) in h_cell pt i
     )
-    (fun #to p -> h_refl (Pointer content p))
-    (fun #to1 #to2 #to3 p1_ p2_ p3_ -> h_trans (Pointer content p1_) (Pointer content p2_) (Pointer content p3_))
+    (fun #to p -> h_refl (Pointer from contents p))
+    (fun #to1 #to2 #to3 p1_ p2_ p3_ -> h_trans (Pointer from contents p1_) (Pointer from contents p2_) (Pointer from contents p3_))
     (Pointer?.p p1)
     (Pointer?.p p2)
 
+abstract
 let unused_in_includes
-  (#value1: Type)
-  (#value2: Type)
+  (#value1: typ)
+  (#value2: typ)
   (h: HS.mem)
   (p1: pointer value1)
   (p2: pointer value2)
@@ -1003,15 +1586,16 @@ let unused_in_includes
   [SMTPatT (unused_in p2 h); SMTPatT (includes p1 p2)]
 = includes_ind
   (fun #v1 #v2 p1 p2 -> unused_in p1 h <==> unused_in p2 h)
-  (fun #k #v p fd -> unused_in_gfield h p fd)
+  (fun l p fd -> unused_in_gfield p fd h)
   (fun #length #value p i -> unused_in_gcell h p i)
   (fun #v p -> ())
   (fun #v1 #v2 #v3 p1 p2 p3 -> ())
   p1 p2
 
+abstract
 let live_includes
-  (#value1: Type)
-  (#value2: Type)
+  (#value1: typ)
+  (#value2: typ)
   (h: HS.mem)
   (p1: pointer value1)
   (p2: pointer value2)
@@ -1021,37 +1605,42 @@ let live_includes
   [SMTPatT (live h p2); SMTPatT (includes p1 p2)]
 = includes_ind
   (fun #v1 #v2 p1 p2 -> live h p1 <==> live h p2)
-  (fun #k #v p fd -> live_gfield h p fd)
+  (fun l p fd -> live_gfield h p fd)
   (fun #length #value p i -> live_gcell h p i)
   (fun #v p -> ())
   (fun #v1 #v2 #v3 p1 p2 p3 -> ())
   p1 p2
 
 abstract let disjoint
-  (#value1: Type)
-  (#value2: Type)
+  (#value1: typ)
+  (#value2: typ)
   (p1: pointer value1)
   (p2: pointer value2)
 : GTot Type0
-= (frameOf p1 <> frameOf p2 \/ as_addr p1 =!= as_addr p2) \/ // disjoint references; see HyperStack.lemma_live_1
-  (Pointer?.from p1 == Pointer?.from p2 /\ Pointer?.content p1 == Pointer?.content p2 /\ path_disjoint (Pointer?.p p1) (Pointer?.p p2))
+= if
+    frameOf p1 = frameOf p2 &&
+    as_addr p1 = as_addr p2
+  then
+    Pointer?.from p1 == Pointer?.from p2 /\
+    Pointer?.contents p1 == Pointer?.contents p2 /\
+    path_disjoint (Pointer?.p p1) (Pointer?.p p2)
+  else
+    True
 
 abstract let disjoint_root
-  (#value1: Type)
-  (#value2: Type)
+  (#value1: typ)
+  (#value2: typ)
   (p1: pointer value1)
   (p2: pointer value2)
 : Lemma
-  (requires (frameOf p1 <> frameOf p2 \/ as_addr p1 =!= as_addr p2))
+  (requires (frameOf p1 <> frameOf p2 \/ as_addr p1 <> as_addr p2))
   (ensures (disjoint p1 p2))
 = ()
 
 abstract let disjoint_gfield
-  (#key: eqtype)
-  (#value: (key -> Tot Type))
-  (p: pointer (DM.t key value))
-  (fd1: key)
-  (fd2: key)
+  (#l: struct_typ)
+  (p: pointer (TStruct l))
+  (fd1 fd2: struct_field l)
 : Lemma
   (requires (fd1 <> fd2))
   (ensures (disjoint (gfield p fd1) (gfield p fd2)))
@@ -1060,8 +1649,8 @@ abstract let disjoint_gfield
 
 abstract let disjoint_gcell
   (#length: UInt32.t)
-  (#value: Type)
-  (p: pointer (array length value))
+  (#value: typ)
+  (p: pointer (TArray length value))
   (i1: UInt32.t {UInt32.v i1 < UInt32.v length})
   (i2: UInt32.t {UInt32.v i2 < UInt32.v length})
 : Lemma
@@ -1071,98 +1660,94 @@ abstract let disjoint_gcell
 = ()
 
 abstract let disjoint_includes
-  (#value1: Type)
-  (#value2: Type)
+  (#value1: typ)
+  (#value2: typ)
   (p1: pointer value1)
   (p2: pointer value2)
-  (#value1': Type)
-  (#value2': Type)
+  (#value1': typ)
+  (#value2': typ)
   (p1': pointer value1')
   (p2': pointer value2')
 : Lemma
   (requires (includes p1 p1' /\ includes p2 p2' /\ disjoint p1 p2))
   (ensures (disjoint p1' p2'))
-= FStar.Classical.or_elim
-    #(frameOf p1 <> frameOf p2 \/ as_addr p1 =!= as_addr p2)
-    #(Pointer?.from p1 == Pointer?.from p2 /\ Pointer?.content p1 == Pointer?.content p2 /\ path_disjoint (Pointer?.p p1) (Pointer?.p p2))
-    #(fun _ -> disjoint p1' p2')
-    (fun h -> ())
-    (fun _ -> path_disjoint_includes (Pointer?.p p1) (Pointer?.p p2) (Pointer?.p p1') (Pointer?.p p2'))
+= if
+    frameOf p1 = frameOf p2 &&
+    as_addr p1 = as_addr p2
+  then
+    path_disjoint_includes (Pointer?.p p1) (Pointer?.p p2) (Pointer?.p p1') (Pointer?.p p2')
+  else
+    ()
 
 abstract let disjoint_ind
   (x:
-    (#value1: Type) ->
-    (#value2: Type) ->
+    (#value1: typ) ->
+    (#value2: typ) ->
     (p1: pointer value1) ->
     (p2: pointer value2 {disjoint p1 p2} ) ->
     GTot Type0)
   (h_root:
-    (#value1: Type) ->
-    (#value2: Type) ->
+    (#value1: typ) ->
+    (#value2: typ) ->
     (p1: pointer value1) ->
-    (p2: pointer value2 { frameOf p1 <> frameOf p2 \/ as_addr p1 =!= as_addr p2 } ) ->
+    (p2: pointer value2 { frameOf p1 <> frameOf p2 \/ as_addr p1 <> as_addr p2 } ) ->
     Lemma (x p1 p2))
   (h_field:
-    (#key: eqtype) ->
-    (#value: (key -> Tot Type)) ->
-    (p: pointer (DM.t key value)) ->
-    (fd1: key) ->
-    (fd2: key { fd1 <> fd2 /\ disjoint (gfield p fd1) (gfield p fd2) } ) ->
+    (#l: struct_typ) ->
+    (p: pointer (TStruct l)) ->
+    (fd1: struct_field l) ->
+    (fd2: struct_field l { fd1 <> fd2 /\ disjoint (gfield p fd1) (gfield p fd2) } ) ->
     Lemma (x (gfield p fd1) (gfield p fd2)))
   (h_cell:
     (#length: UInt32.t) ->
-    (#value: Type) ->
-    (p: pointer (array length value)) ->
+    (#value: typ) ->
+    (p: pointer (TArray length value)) ->
     (i1: UInt32.t {UInt32.v i1 < UInt32.v length}) ->
     (i2: UInt32.t {UInt32.v i2 < UInt32.v length /\ UInt32.v i1 <> UInt32.v i2 /\ disjoint (gcell p i1) (gcell p i2) }) ->
     Lemma (x (gcell p i1) (gcell p i2))
   )
   (h_includes:
-    (#value1: Type) ->
-    (#value2: Type) ->
+    (#value1: typ) ->
+    (#value2: typ) ->
     (p1: pointer value1) ->
     (p2: pointer value2) ->
-    (#value1': Type) ->
-    (#value2': Type) ->
+    (#value1': typ) ->
+    (#value2': typ) ->
     (p1': pointer value1' {includes p1 p1'}) ->
     (p2': pointer value2' {includes p2 p2' /\ disjoint p1 p2 /\ disjoint p1' p2' /\ x p1 p2}) ->
     Lemma (x p1' p2'))
-  (#value1: Type)
-  (#value2: Type)
+  (#value1: typ)
+  (#value2: typ)
   (p1: pointer value1)
   (p2: pointer value2 { disjoint p1 p2 } )
 : Lemma (x p1 p2)
-= FStar.Classical.or_elim
-    #(frameOf p1 <> frameOf p2 \/ as_addr p1 =!= as_addr p2)
-    #(Pointer?.from p1 == Pointer?.from p2 /\ Pointer?.content p1 == Pointer?.content p2 /\ path_disjoint (Pointer?.p p1) (Pointer?.p p2))
-    #(fun _ -> x p1 p2)
-    (fun _ ->
-      h_root p1 p2)
-    (fun _ ->
-      let from: Type = Pointer?.from p1 in
-      let (content1: HS.reference from ) = Pointer?.content p1 in
-      let (content2: HS.reference from ) = Pointer?.content p2 in
-      assert (content1 == content2);
-      path_disjoint_ind
-	(fun #v1 #v2 p1_ p2_ -> x (Pointer content1 p1_) (Pointer content1 p2_))
-	(fun #through #to1 #to2 p s1 s2 ->
-	   match s1 with
-	   | StepField ke va fd1 ->
-	     let (StepField _ _ fd2) = s2 in
-	     h_field #ke #va (Pointer content1 p) fd1 fd2
-	   | StepCell le va i1 ->
-	     let (StepCell _ _ i2) = s2 in
-	     h_cell #le #va (Pointer content1 p) i1 i2
-	)
-	(fun #v1 #v2 p1_ p2_ #v1' #v2' p1' p2' -> h_includes (Pointer content1 p1_) (Pointer content1 p2_) (Pointer content1 p1') (Pointer content1 p2'))
-	(Pointer?.p p1)
-	(Pointer?.p p2);
-       assert (x p1 p2)
-     )
+= if
+    frameOf p1 = frameOf p2 &&
+    as_addr p1 = as_addr p2
+  then
+    let (Pointer from contents _) = p1 in
+    path_disjoint_ind
+      (fun #v1 #v2 p1_ p2_ -> x (Pointer from contents p1_) (Pointer from contents p2_))
+      (fun #through #to1 #to2 p s1 s2 ->
+         match s1 with
+         | StepField l fd1 ->
+           let (StepField _ fd2) = s2 in
+           h_field #l (Pointer from contents p) fd1 fd2
+         | StepCell le va i1 ->
+           let (StepCell _ _ i2) = s2 in
+           h_cell #le #va (Pointer from contents p) i1 i2
+      )
+      (fun #v1 #v2 p1_ p2_ #v1' #v2' p1' p2' -> h_includes (Pointer from contents p1_) (Pointer from contents p2_) (Pointer from contents p1') (Pointer from contents p2'))
+      (Pointer?.p p1)
+      (Pointer?.p p2);
+      assert (x p1 p2)
+  else
+    h_root p1 p2
 
+abstract
 let disjoint_sym
-  (#value1: Type)
-  (#value2: Type)
+  (#value1: typ)
+  (#value2: typ)
   (p1: pointer value1)
   (p2: pointer value2)
 : Lemma
@@ -1171,14 +1756,15 @@ let disjoint_sym
 = disjoint_ind
   (fun #v1 #v2 p1 p2 -> disjoint p2 p1)
   (fun #v1 #v2 p1 p2 -> disjoint_root p2 p1)
-  (fun #k #v p fd1 fd2 -> disjoint_gfield p fd2 fd1)
+  (fun #l p fd1 fd2 -> disjoint_gfield p fd2 fd1)
   (fun #le #va p i1 i2 -> disjoint_gcell p i2 i1)
   (fun #v1 #v2 p1 p2 #v1' #v2' p1' p2' -> disjoint_includes p2 p1 p2' p1')
   p1 p2
 
+abstract
 let disjoint_sym'
-  (#value1: Type)
-  (#value2: Type)
+  (#value1: typ)
+  (#value2: typ)
   (p1: pointer value1)
   (p2: pointer value2)
 : Lemma
@@ -1188,21 +1774,55 @@ let disjoint_sym'
 = FStar.Classical.move_requires (disjoint_sym #value1 #value2 p1) p2;
   FStar.Classical.move_requires (disjoint_sym #value2 #value1 p2) p1
 
+abstract
 let disjoint_includes_l #a #as #a' (x: pointer a) (subx:pointer as) (y:pointer a') : Lemma
   (requires (includes x subx /\ disjoint x y))
   (ensures  (disjoint subx y))
   [SMTPatT (disjoint subx y); SMTPatT (includes x subx)]
   = disjoint_includes x y subx y
 
+abstract
 let disjoint_includes_l_swap #a #as #a' (x:pointer a) (subx:pointer as) (y:pointer a') : Lemma
   (requires (includes x subx /\ disjoint x y))
   (ensures  (disjoint y subx))
   [SMTPatT (disjoint y subx); SMTPatT (includes x subx)]
   = ()
 
-let live_disjoint
-  (#value1: Type)
-  (#value2: Type)
+abstract
+let live_not_equal_disjoint
+  (#t: typ)
+  (h: HS.mem)
+  (p1 p2: pointer t)
+: Lemma
+  (requires (live h p1 /\ live h p2 /\ equal p1 p2 == false))
+  (ensures (disjoint p1 p2))
+= if
+    frameOf p1 = frameOf p2 &&
+    as_addr p1 = as_addr p2
+  then begin
+    let c1 = greference_of p1 in
+    let c2 = greference_of p2 in
+    HS.lemma_same_addrs_same_types_same_refs h c1 c2;
+    not_path_equal_path_disjoint_same_type p1.p p2.p
+  end else
+    disjoint_root p1 p2
+
+abstract
+let live_unused_in_disjoint_strong
+  (#value1: typ)
+  (#value2: typ)
+  (h: HS.mem)
+  (p1: pointer value1)
+  (p2: pointer value2)
+: Lemma
+  (requires (live h p1 /\ unused_in p2 h))
+  (ensures (frameOf p1 <> frameOf p2 \/ as_addr p1 <> as_addr p2))
+= ()
+
+abstract
+let live_unused_in_disjoint
+  (#value1: typ)
+  (#value2: typ)
   (h: HS.mem)
   (p1: pointer value1)
   (p2: pointer value2)
@@ -1210,14 +1830,15 @@ let live_disjoint
   (requires (live h p1 /\ unused_in p2 h))
   (ensures (disjoint p1 p2))
   [SMTPatT (disjoint p1 p2); SMTPatT (live h p1)]
-= disjoint_root p1 p2
+= live_unused_in_disjoint_strong h p1 p2;
+  disjoint_root p1 p2
 
 (*** The modifies clause *)
 
 // private // in fact, we have to expose this type, otherwise unification problems will appear everywhere
 noeq type apointer =
 | APointer:
-  (a: Type) ->
+  (a: typ) ->
   (p: pointer a) ->
   apointer
 
@@ -1255,7 +1876,7 @@ let set_amem
 = TSet.mem a (Set?.pointers s)
 
 let set_mem
-  (#a: Type)
+  (#a: typ)
   (p: pointer a)
   (s: set)
 : GTot Type0
@@ -1272,7 +1893,7 @@ abstract let set_amem_empty
 = ()
 
 abstract let set_singleton
-  (#a: Type)
+  (#a: typ)
   (x: pointer a)
 : Tot set
 =
@@ -1281,7 +1902,7 @@ abstract let set_singleton
   Set pointers (Ghost.elift1 f (Ghost.hide ()))
 
 abstract let set_amem_singleton
-  (#a: Type)
+  (#a: typ)
   (x: pointer a)
   (x': apointer)
 : Lemma
@@ -1398,9 +2019,9 @@ let set_subset_includes
   )
 
 let set_includes_singleton
-  (#a1: Type)
+  (#a1: typ)
   (p1: pointer a1)
-  (#a2: Type)
+  (#a2: typ)
   (p2: pointer a2)
 : Lemma
   (requires (p1 `includes` p2))
@@ -1425,6 +2046,89 @@ let modifies
     live h2 (APointer?.p a') /\ gread h1 (APointer?.p a') == gread h2 (APointer?.p a')
   ))
 
+(*
+private
+assume val
+modifies_ref_not_mem
+  (r: HH.rid)
+  (s: Set.set nat)
+  (h1 h2: HS.mem)
+  (#t: typ)
+  (p: pointer t)
+: Lemma
+  (requires (
+    HS.modifies_ref r s h1 h2 /\
+    frameOf p == r /\
+    (~ (Set.mem (as_addr p) s)) /\
+    live h1 p
+  ))
+  (ensures (
+    live h1 p /\
+    live h2 p /\ (
+    let r = reference_of h1 p in (
+    reference_of h2 p == reference_of h1 p /\
+    HS.sel h1 r == HS.sel h2 r
+  ))))
+  [SMTPat (HS.modifies_ref r s h1 h2); SMTPat (live h1 p)]
+
+private
+assume val
+modifies_ref_not_mem
+  (s: Set.set HH.rid)
+  (h1 h2: HS.mem)
+  (#t: typ)
+  (p: pointer t)
+: Lemma
+  (requires (
+    HS.modifies s h1 h2 /\
+    (~ (Set.mem (frameOf p) s)) /\
+    live h1 p
+  ))
+  (ensures (
+    live h1 p /\
+    live h2 p /\ (
+    let r = reference_of h1 p in (
+    reference_of h2 p == reference_of h1 p /\
+    HS.sel h1 r == HS.sel h2 r
+  ))))
+  [SMTPat (HS.modifies s h1 h2); SMTPat (live h1 p)]
+
+private
+assume val modifies_equiv
+  (r: HH.rid)
+  (s: set)
+  (h1 h2: HS.mem)
+: Lemma
+  (modifies r s h1 h2 <==> (
+  HS.modifies_ref r (Ghost.reveal (Set?.addrs s)) h1 h2 /\ (
+  forall (a': apointer) . (
+  let p' = APointer?.p a' in ((
+    frameOf p' == r /\
+    live h1 p'
+  ) ==> (
+    let ref' = reference_of h1 p' in ((
+      forall (a: apointer) . (
+      let p = APointer?.p a in ((
+        TSet.mem a (Set?.pointers s) /\
+        frameOf p == r /\
+        as_addr p == as_addr p' /\
+        Pointer?.from p == Pointer?.from p' /\
+        Pointer?.contents p == Pointer?.contents p' /\
+	reference_of h1 p == ref'
+      ) ==>
+      path_disjoint (Pointer?.p p) (Pointer?.p p')
+    ))) ==>
+    HS.contains h2 ref' /\ ((
+      live h2 p' /\
+      reference_of h2 p' == ref'
+    ) ==> (
+      let (| _, c1 |) = HS.sel h1 ref' in
+      let (| _, c2 |) = HS.sel h2 ref' in
+      path_sel c1 (Pointer?.p p') == path_sel c2 (Pointer?.p p')
+  )))))))))
+  [SMTPat (modifies r s h1 h2)]
+*)
+
 abstract
 let modifies_modifies_ref
   (r: HH.rid)
@@ -1436,7 +2140,7 @@ let modifies_modifies_ref
     exists (rs: Set.set nat) .
     HS.modifies_ref r rs h1 h2 /\ (
     forall (x: nat) . Set.mem x rs <==> (
-    exists (a: Type) (p: pointer a) .
+    exists (a: typ) (p: pointer a) .
     set_mem p s /\
     as_addr p == x
   ))))
@@ -1447,7 +2151,7 @@ let modifies_elim
   (r: HH.rid)
   (s: set)
   (h1 h2: HS.mem)
-  (#a': Type)
+  (#a': typ)
   (p': pointer a')
 : Lemma
   (requires (
@@ -1474,11 +2178,11 @@ let modifies_intro
   (requires (
     HS.modifies_ref r rs h1 h2 /\ (
       forall (n: nat) . Set.mem n rs <==> (
-      exists (a: Type) (p: pointer a) .
+      exists (a: typ) (p: pointer a) .
       set_mem p s /\
       as_addr p == n
     )) /\ (
-      forall (a': Type) (p': pointer a' { frameOf p' == r /\ live h1 p' } ) . (
+      forall (a': typ) (p': pointer a' { frameOf p' == r /\ live h1 p' } ) . (
         forall (ap: apointer { frameOf (APointer?.p ap) == r /\ set_amem ap s } ) .
         disjoint (APointer?.p ap) p'
       ) ==> (
@@ -1549,7 +2253,7 @@ let modifies_set_includes
 let modifies_ptr_0 rid h h' =
   modifies rid set_empty h h'
 
-let modifies_ptr_1 (#t:Type) rid (b:pointer t) h h' = //would be good to drop the rid argument on these, since they can be computed from the pointers
+let modifies_ptr_1 (#t:typ) rid (b:pointer t) h h' = //would be good to drop the rid argument on these, since they can be computed from the pointers
   modifies rid (set_singleton b) h h'
 
 let modifies_ptr_0_0 rid h0 h1 h2 :
@@ -1570,7 +2274,7 @@ abstract let modifies_0 h0 h1 =
 (* This one is very generic: it says
  * - some references have changed in the frame of b, but
  * - among all pointers in this frame, b is the only one that changed. *)
-abstract let modifies_1 (#a:Type) (b:pointer a) h0 h1 =
+abstract let modifies_1 (#a:typ) (b:pointer a) h0 h1 =
   let rid = frameOf b in
   HS.modifies_one rid h0 h1 /\ modifies_ptr_1 rid b h0 h1
 
@@ -1582,7 +2286,7 @@ let modifies_0_intro h0 h1 : Lemma
   (ensures  (modifies_0 h0 h1))
   = ()
 
-let modifies_1_intro (#a:Type) (b:pointer a) h0 h1 : Lemma
+let modifies_1_intro (#a:typ) (b:pointer a) h0 h1 : Lemma
   (requires (let rid = frameOf b in
   HS.modifies_one rid h0 h1 /\ modifies_ptr_1 rid b h0 h1))
   (ensures  (modifies_1 b h0 h1))
@@ -1595,17 +2299,65 @@ let  modifies_0_reveal h0 h1 : Lemma
   (ensures  (HS.modifies_one h0.HS.tip h0 h1 /\ modifies_ptr_0 h0.HS.tip h0 h1 /\ h0.HS.tip=h1.HS.tip))
   = ()
 
-let modifies_1_reveal (#a:Type) (b:pointer a) h0 h1 : Lemma
+let modifies_1_reveal (#a:typ) (b:pointer a) h0 h1 : Lemma
   (requires (modifies_1 b h0 h1))
   (ensures  (let rid = frameOf b in HS.modifies_one rid h0 h1 /\ modifies_ptr_1 rid b h0 h1))
   = ()
 
+(*
+#reset-options "--z3rlimit 32"
+
+assume val fresh_frame_aref_live_at
+  (h0 h1: HS.mem)
+  (a: HS.aref)
+  (t: Type0)
+: Lemma
+  (requires (
+    HS.fresh_frame h0 h1 /\
+    HS.aref_live_at h0 a t
+  ))
+  (ensures (
+    HS.aref_live_at h0 a t /\
+    HS.frameOf_aref a <> h1.HS.tip /\
+    HS.aref_live_at h1 a t /\ (
+    let r = HS.reference_of h0 a t in (
+    r == HS.reference_of h1 a t /\
+    HS.frameOf r == HS.frameOf_aref a /\
+    HS.as_addr r == HS.aref_as_addr a /\
+    HS.sel h0 r == HS.sel h1 r
+  ))))
+  [SMTPat (HS.fresh_frame h0 h1); SMTPat (HS.aref_live_at h0 a t)]
+
+assume val popped_aref_live_at
+  (h0 h1: HS.mem)
+  (a: HS.aref)
+  (t: Type0)
+: Lemma
+  (requires (
+    HS.popped h0 h1 /\
+    HS.aref_live_at h0 a t /\
+    HS.frameOf_aref a <> h0.HS.tip
+  ))
+  (ensures (
+    HS.aref_live_at h0 a t /\
+    HS.aref_live_at h1 a t /\ (
+    let r = HS.reference_of h0 a t in (
+    r == HS.reference_of h1 a t /\
+    HS.frameOf r == HS.frameOf_aref a /\
+    HS.as_addr r == HS.aref_as_addr a /\
+    HS.sel h0 r == HS.sel h1 r  
+  ))))
+  [SMTPat (HS.popped h0 h1); SMTPat (HS.aref_live_at h0 a t)]
+*)
+
 (* STStack effect specific lemmas *)
-let lemma_ststack_1 (#a:Type) (b:pointer a) h0 h1 h2 h3 : Lemma
-  (requires (live h0 b /\ HS.fresh_frame h0 h1 /\ modifies_1 b h1 h2 /\ HS.popped h2 h3))
+let lemma_ststack_1 (#a:typ) (b:pointer a) h0 h1 h2 h3 : Lemma
+  (requires (live h0 b /\ HS.fresh_frame h0 h1 /\ modifies_1 b h1 h2 /\ HS.popped h2 h3 ))
   (ensures  (modifies_1 b h0 h3))
   [SMTPatT (modifies_1 b h1 h2); SMTPatT (HS.fresh_frame h0 h1); SMTPatT (HS.popped h2 h3)]
-  = ()
+= ()
+
+//  assume (modifies_1 b h0 h3)
 
 (** Transitivity lemmas *)
 let modifies_0_trans h0 h1 h2 : Lemma
@@ -1614,7 +2366,7 @@ let modifies_0_trans h0 h1 h2 : Lemma
   [SMTPatT (modifies_0 h0 h1); SMTPatT (modifies_0 h1 h2)]
   = ()
 
-let modifies_1_trans (#a:Type) (b:pointer a) h0 h1 h2 : Lemma
+let modifies_1_trans (#a:typ) (b:pointer a) h0 h1 h2 : Lemma
   (requires (modifies_1 b h0 h1 /\ modifies_1 b h1 h2))
   (ensures (modifies_1 b h0 h2))
   [SMTPatT (modifies_1 b h0 h1); SMTPatT (modifies_1 b h1 h2)]
@@ -1627,17 +2379,18 @@ val modifies_0_0: h0:HS.mem -> h1:HS.mem -> h2:HS.mem -> Lemma
   [SMTPatT (modifies_0 h0 h1); SMTPatT (modifies_0 h1 h2)]
 let modifies_0_0 h0 h1 h2 = ()
 
-let modifies_0_1 (#a:Type) (b:pointer a) h0 h1 h2 : Lemma
+abstract
+let modifies_0_1 (#a:typ) (b:pointer a) h0 h1 h2 : Lemma
   (requires (unused_in b h0 /\ modifies_0 h0 h1 /\ live h1 b /\ modifies_1 b h1 h2))
   (ensures  (modifies_0 h0 h2))
   [SMTPatT (modifies_0 h0 h1); SMTPatT (modifies_1 b h1 h2)]
-  = ()
+= ()
 
 (** Concrete allocators, getters and setters *)
 
 abstract let screate
-  (#value:Type)
-  (s: value)
+  (#value:typ)
+  (s: type_of_typ value)
 : StackInline (pointer value)
   (requires (fun h -> True))
   (ensures (fun (h0:HS.mem) b h1 ->
@@ -1647,10 +2400,10 @@ abstract let screate
      /\ modifies_0 h0 h1
      /\ Map.domain h1.HS.h == Map.domain h0.HS.h
      /\ gread h1 b == s))
-= let content: HS.reference value =
-     HST.salloc s
+= let content: HS.reference pointer_ref_contents =
+     HST.salloc (| value, s |)
   in
-  Pointer content PathBase
+  Pointer value (HS.aref_of content) PathBase
 
 // TODO: move to HyperStack?
 private let domain_upd (#a:Type) (h:HS.mem) (x:HS.reference a{HS.live_region h x.HS.id}) (v:a) : Lemma
@@ -1661,9 +2414,9 @@ private let domain_upd (#a:Type) (h:HS.mem) (x:HS.reference a{HS.live_region h x
     Set.lemma_equal_intro (Map.domain m) (Map.domain m')
 
 abstract let ecreate
-  (#t:Type)
+  (#t:typ)
   (r:HH.rid)
-  (s: t)
+  (s: type_of_typ t)
 : ST (pointer t)
   (requires (fun h -> HS.is_eternal_region r))
   (ensures (fun (h0:HS.mem) b h1 -> unused_in b h0
@@ -1673,28 +2426,27 @@ abstract let ecreate
     /\ HS.modifies (Set.singleton r) h0 h1
     /\ HS.modifies_ref r Set.empty h0 h1
     /\ gread h1 b == s
-    /\ ~(memory_managed b)))
+    /\ ~(is_mm b)))
 = let h0 = HST.get() in
-  let content: HS.reference t = ralloc r s in
-  let b = Pointer content PathBase in
-  let h1 = HST.get() in
-  domain_upd h0 content s;
-  b
+  let content: HS.reference pointer_ref_contents =
+     HST.ralloc r (| t, s |)
+  in
+  domain_upd h0 content (| t, s |) ;
+  Pointer t (HS.aref_of content) PathBase
 
 abstract let field
- (#key: eqtype)
- (#value: (key -> Tot Type))
- (p: pointer (DM.t key value))
- (fd: key)
-: ST (pointer (value fd))
+ (#l: struct_typ)
+ (p: pointer (TStruct l))
+ (fd: struct_field l)
+: ST (pointer (typ_of_struct_field l fd))
   (requires (fun h -> live h p))
   (ensures (fun h0 p' h1 -> h0 == h1 /\ p' == gfield p fd))
 = _field p fd
 
 abstract let cell
  (#length: UInt32.t)
- (#value: Type)
- (p: pointer (array length value))
+ (#value: typ)
+ (p: pointer (TArray length value))
  (i: UInt32.t {UInt32.v i < UInt32.v length})
 : ST (pointer value)
   (requires (fun h -> live h p))
@@ -1702,50 +2454,43 @@ abstract let cell
 = _cell p i
 
 abstract let read
- (#value: Type)
+ (#value: typ)
  (p: pointer value)
-: ST value
+: ST (type_of_typ value)
   (requires (fun h -> live h p))
   (ensures (fun h0 v h1 -> live h0 p /\ h0 == h1 /\ v == gread h0 p))
-= let (Pointer content p') = p in
-  path_sel (!content) p'
+= let h = HST.get () in
+  let r = reference_of h p in
+  let (| _ , c |) = !r in
+  path_sel c (Pointer?.p p)
 
-private val hs_upd_path_upd: #a:Type -> b:pointer a -> z:a
-  -> h0:HS.mem -> Lemma
-  (requires (live h0 b))
-  (ensures (live h0 b /\
-    modifies_1 b h0  (HS.upd h0 (Pointer?.content b) (path_upd (HS.sel h0 (Pointer?.content b)) (Pointer?.p b) z))))
-  [SMTPat (HS.upd h0 (Pointer?.content b) (path_upd (HS.sel h0 (Pointer?.content b)) (Pointer?.p b) z))]
-let hs_upd_path_upd #a b z h0 =
-  let s = set_singleton b in
-  let (ap: apointer { set_amem ap s } ) = APointer a b in
-  ()
-
-abstract val write: #a:Type -> b:pointer a -> z:a -> Stack unit
+abstract val write: #a:typ -> b:pointer a -> z:(type_of_typ a) -> Stack unit
   (requires (fun h -> live h b))
   (ensures (fun h0 _ h1 -> live h0 b /\ live h1 b
     /\ modifies_1 b h0 h1
     /\ gread h1 b == z ))
 let write #a b z =
-  let s0 = !b.content in
-  let s = path_upd s0 (Pointer?.p b) z in
-  b.content := s
+  let h0 = HST.get () in
+  let r = reference_of h0 b in
+  let (| t , c0 |) = !r in
+  let c1 = path_upd c0 (Pointer?.p b) z in
+  r := (| t, c1 |)
 
 (** Lemmas and patterns *)
 
-let modifies_one_trans_1 (#a:Type) (b:pointer a) (h0:HS.mem) (h1:HS.mem) (h2:HS.mem): Lemma
+let modifies_one_trans_1 (#a:typ) (b:pointer a) (h0:HS.mem) (h1:HS.mem) (h2:HS.mem): Lemma
   (requires (HS.modifies_one (frameOf b) h0 h1 /\ HS.modifies_one (frameOf b) h1 h2))
   (ensures (HS.modifies_one (frameOf b) h0 h2))
   [SMTPatT (HS.modifies_one (frameOf b) h0 h1); SMTPatT (HS.modifies_one (frameOf b) h1 h2)]
   = ()
 
-val no_upd_lemma_0: #t:Type -> h0:HS.mem -> h1:HS.mem -> b:pointer t -> Lemma
+val no_upd_lemma_0: #t:typ -> h0:HS.mem -> h1:HS.mem -> b:pointer t -> Lemma
   (requires (live h0 b /\ modifies_0 h0 h1))
   (ensures  (live h0 b /\ live h1 b /\ equal_values h0 b h1 b))
   [SMTPatT (modifies_0 h0 h1); SMTPatT (live h0 b)]
 let no_upd_lemma_0 #t h0 h1 b = ()
 
-val no_upd_lemma_1: #t:Type -> #t':Type -> h0:HS.mem -> h1:HS.mem -> a:pointer t -> b:pointer t' -> Lemma
+val no_upd_lemma_1: #t:typ -> #t':typ -> h0:HS.mem -> h1:HS.mem -> a:pointer t -> b:pointer t' -> Lemma
   (requires (live h0 b /\ disjoint a b /\ modifies_1 a h0 h1))
   (ensures  (live h0 b /\ live h1 b /\ equal_values h0 b h1 b))
   [SMTPatOr [ [ SMTPatT (modifies_1 a h0 h1); SMTPatT (gread h1 b) ] ; [ SMTPatT (modifies_1 a h0 h1); SMTPatT (live h0 b) ] ] ]
@@ -1754,13 +2499,13 @@ let no_upd_lemma_1 #t #t' h0 h1 a b =
   then modifies_elim (frameOf a) (set_singleton a) h0 h1 b
   else ()
 
-val no_upd_fresh: #t:Type -> h0:HS.mem -> h1:HS.mem -> a:pointer t -> Lemma
+val no_upd_fresh: #t:typ -> h0:HS.mem -> h1:HS.mem -> a:pointer t -> Lemma
   (requires (live h0 a /\ HS.fresh_frame h0 h1))
   (ensures  (live h0 a /\ live h1 a /\ equal_values h0 a h1 a))
   [SMTPatT (live h0 a); SMTPatT (HS.fresh_frame h0 h1)]
 let no_upd_fresh #t h0 h1 a = ()
 
-val no_upd_popped: #t:Type -> h0:HS.mem -> h1:HS.mem -> b:pointer t -> Lemma
+val no_upd_popped: #t:typ -> h0:HS.mem -> h1:HS.mem -> b:pointer t -> Lemma
   (requires (live h0 b /\ frameOf b <> h0.HS.tip /\ HS.popped h0 h1))
   (ensures  (live h0 b /\ live h1 b /\ equal_values h0 b h1 b))
   [SMTPatT (live h0 b); SMTPatT (HS.popped h0 h1)]
@@ -1772,7 +2517,7 @@ let lemma_modifies_sub_1 #t h0 h1 (b:pointer t) : Lemma
   [SMTPatT (live h0 b); SMTPatT (modifies_1 b h0 h1)]
   = ()
 
-let modifies_substruct_1 (#tsub #ta:Type) h0 h1 (sub:pointer tsub) (a:pointer ta) : Lemma
+let modifies_substruct_1 (#tsub #ta:typ) h0 h1 (sub:pointer tsub) (a:pointer ta) : Lemma
   (requires (live h0 a /\ modifies_1 sub h0 h1 /\ live h1 sub /\ includes a sub))
   (ensures  (modifies_1 a h0 h1 /\ live h1 a))
   [SMTPatT (modifies_1 sub h0 h1); SMTPatT (includes a sub)]
@@ -1781,19 +2526,19 @@ let modifies_substruct_1 (#tsub #ta:Type) h0 h1 (sub:pointer tsub) (a:pointer ta
   set_includes_singleton a sub;
   modifies_set_includes (frameOf a) s1 s2 h0 h1
 
-let modifies_popped_1' (#t:Type) (a:pointer t) h0 h1 h2 h3 : Lemma
+let modifies_popped_1' (#t:typ) (a:pointer t) h0 h1 h2 h3 : Lemma
   (requires (live h0 a /\ HS.fresh_frame h0 h1 /\ HS.popped h2 h3 /\ modifies_1 a h1 h2))
   (ensures  (modifies_1 a h0 h3))
   [SMTPatT (HS.fresh_frame h0 h1); SMTPatT (HS.popped h2 h3); SMTPatT (modifies_1 a h1 h2)]
   = ()
 
-let live_popped (#t:Type) (b:pointer t) h0 h1 : Lemma
+let live_popped (#t:typ) (b:pointer t) h0 h1 : Lemma
   (requires (HS.popped h0 h1 /\ live h0 b /\ frameOf b <> h0.HS.tip))
   (ensures  (live h1 b))
   [SMTPatT (HS.popped h0 h1); SMTPatT (live h0 b)]
   = ()
 
-let live_fresh (#t:Type) (b:pointer t) h0 h1 : Lemma
+let live_fresh (#t:typ) (b:pointer t) h0 h1 : Lemma
   (requires (HS.fresh_frame h0 h1 /\ live h0 b))
   (ensures  (live h1 b))
   [SMTPatT (HS.fresh_frame h0 h1); SMTPatT (live h0 b)]
@@ -1811,7 +2556,7 @@ abstract
 let modifies_other_regions
   (rs: Set.set HH.rid)
   (h0 h1: HS.mem)
-  (#a: Type)
+  (#a: typ)
   (p: pointer a)
 : Lemma
   (requires (HS.modifies rs h0 h1 /\ (~ (Set.mem (frameOf p) rs)) /\ live h0 p))
@@ -1822,7 +2567,7 @@ abstract
 let modifies_one_other_region
   (r: HH.rid)
   (h0 h1: HS.mem)
-  (#a: Type)
+  (#a: typ)
   (p: pointer a)
 : Lemma
   (requires (HS.modifies_one r h0 h1 /\ frameOf p <> r /\ live h0 p))
